finished tweaking inline proof

theories/L6_PCPS/inline_correct.v
@@ -124,107 +124,6 @@ End Inline_Eq.
 
 Opaque bind ret.
 
-Definition Range (x1 x2 : positive) : Ensemble var := fun z => x1 <= z < x2.
-
-Lemma Disjoint_Range (x1 x2 x1' x2' : positive) :
-  x2 <= x1' ->
-  Disjoint _ (Range x1 x2) (Range x1' x2').
-Proof.
-  intros Hleq. constructor. intros x Hin. inv Hin.
-  unfold Range, Ensembles.In in *. simpl in *. zify. omega.
-Qed.    
-
-Lemma Range_Subset (x1 x2 x1' x2' : positive) :
-  x1 <= x1' ->
-  x2' <= x2 ->
-  Range x1' x2' \subset Range x1 x2.
-Proof.
-  intros H1 H2. intros z Hin. unfold Range, Ensembles.In in *.
-  inv Hin. zify. omega.
-Qed.
-          
-Lemma fresh_Range S (x1 x2 : positive) :
-  fresh S x1 ->
-  Range x1 x2 \subset S.
-Proof.
-  intros Hin z Hin'. inv Hin'. eapply Hin. eassumption.
-Qed.
-
-(** Spec for [get_name] *)
-Lemma get_name_fresh A S y str :
-  {{ fun _ (s : comp_data * A) => fresh S (next_var (fst s)) }}
-    get_name y str
-  {{ fun (r: unit) s x s' =>
-       x \in S /\
-       x \in Range (next_var (fst s)) (next_var (fst s')) /\
-       (next_var (fst s) < next_var (fst s')) /\
-       fresh (S \\ [set x]) (next_var (fst s'))      
-  }}.  
-Proof. 
-  eapply pre_post_mp_l.
-  eapply bind_triple. now eapply get_triple.  
-  intros [[] w1] [[] w2].
-  eapply pre_post_mp_l. simpl.
-  eapply bind_triple. now eapply put_triple.
-  intros x [r3 w3].
-  eapply return_triple. 
-  intros ? [r4 w4] H2. inv H2. intros [H1 H2]. inv H1; inv H2. intros.
-  split. eapply H. reflexivity. split. unfold Range, Ensembles.In. simpl. zify. omega.
-  simpl. split. zify; omega.
-  intros z Hin. constructor. eapply H; eauto. zify. omega.
-  intros Hc. inv Hc. zify; omega.
-Qed.
-
-Lemma get_names_lst_fresh A S ns str :
-  {{ fun _ (s : comp_data * A) => fresh S (next_var (fst s)) }}
-    get_names_lst ns str
-  {{ fun (r: unit) s xs s' =>
-       NoDup xs /\ List.length xs = List.length ns /\
-       FromList xs \subset S /\
-       FromList xs \subset Range (next_var (fst s)) (next_var (fst s')) /\
-       (next_var (fst s) <= next_var (fst s')) /\
-       fresh (S \\ FromList xs) (next_var (fst s')) }}.  
-Proof.
-  unfold get_names_lst. revert S; induction ns; intros S.
-  - simpl. eapply return_triple.
-    intros. repeat normalize_sets. split; eauto. sets. now constructor. split; eauto.
-    split. now sets. split. sets. split. reflexivity. eassumption.
-  - simpl. eapply bind_triple. eapply get_name_fresh.
-    intros x w.
-    eapply bind_triple. eapply frame_rule. eapply frame_rule. eapply frame_rule. eapply IHns.
-    intros xs w'. eapply return_triple. intros. destructAll.
-    repeat normalize_sets. split; [| split; [| split; [| split; [| split ]]]].
-    + constructor; eauto. intros Hc. eapply H4 in Hc. inv Hc. now eauto.
-    + simpl. congruence.
-    + eapply Union_Included. sets. eapply Included_trans. eapply H4. sets.
-    + eapply Union_Included. eapply Singleton_Included.
-      eapply Range_Subset; [| | eassumption ]. reflexivity. zify. omega.
-      eapply Included_trans. eassumption. eapply Range_Subset. zify; omega. reflexivity.
-    + zify; omega.
-    + rewrite <- Setminus_Union. eassumption.
-Qed.
-
-Fixpoint funname_in_exp (e : exp) : Ensemble var :=
-  match e with
-  | Econstr _ _ _ e
-  | Eproj _ _ _ _ e
-  | Eletapp _ _ _ _ e
-  | Eprim _ _ _ e => funname_in_exp e
-  | Ecase _ P =>
-    (fix aux P :=
-       match P with
-       | [] => Empty_set _
-       | (c, e) :: P => funname_in_exp e :|: aux P
-       end) P      
-  | Efun B e => funname_in_fundefs B :|: name_in_fundefs B :|: funname_in_exp e
-  | Eapp _ _ _ 
-  | Ehalt _ => Empty_set _
-  end
-with funname_in_fundefs (B : fundefs) : Ensemble var :=
-       match B with
-       | Fcons _ _ _ e B => funname_in_exp e :|: funname_in_fundefs B
-       | Fnil => Empty_set var
-       end.
   
 Section Inline_correct.
 
@@ -249,103 +148,7 @@ Section Inline_correct.
            (Eletapp_OOT' : remove_steps_letapp_OOT' cenv P1 P1).
 
   
-  
-  Definition occurs_free_fun_map (fm : fun_map) : Ensemble var :=
-    fun x => exists f ft xs e, fm ! f = Some (ft, xs, e) /\ x \in occurs_free e \\ FromList xs.
-
-  Definition bound_var_fun_map (fm : fun_map) : Ensemble var :=
-    fun x => exists f ft xs e, fm ! f = Some (ft, xs, e) /\ x \in bound_var e \\ funname_in_exp e :|: FromList xs.
-
-  Definition bound_var_fun_map' (fm : fun_map) : Ensemble var :=
-    fun x => exists f ft xs e, fm ! f = Some (ft, xs, e) /\ x \in bound_var e :|: FromList xs.
-
-  
-  Fixpoint fun_map_inv' (k : nat) (S : Ensemble var) (fm : fun_map) (rho1 rho2 : env) (i : nat) (sig : subst) : Prop :=
-    forall f ft xs e rhoc B f',
-      f \in S ->
-      fm ! f = Some (ft, xs, e) ->
-      rho1 ! f = Some (Vfun rhoc B f') ->
-      find_def f B = Some (ft, xs, e) /\ f = f' /\
-      (* eq_env_P (occurs_free_fun_map fm) rho1 (def_funs B B rhoc rhoc) *)
-      preord_env_P_inj cenv PG (occurs_free e \\ FromList xs) i (apply_r sig) (def_funs B B rhoc rhoc) rho2 /\
-      (* sub_map (def_funs B B rhoc rhoc) rho1 /\ *)
-      (* Disjoint _ (bound_var e) (name_in_fundefs B) /\ *)
-      (* Disjoint _ (FromList xs) (name_in_fundefs B) /\ *)
-      (* Disjoint _ S (occurs_free e \\ FromList xs) /\ *)
-      match k with
-      | 0%nat => True
-      | S k => fun_map_inv' k (occurs_free e \\ FromList xs) fm (def_funs B B rhoc rhoc) rho2 i sig
-      end.
-
-  Definition fun_map_inv (k : nat) (S : Ensemble var) (fm : fun_map) (rho1 rho2 : env) (i : nat) (sig : subst) : Prop :=
-    forall f ft xs e rhoc B f',
-      f \in S ->
-      fm ! f = Some (ft, xs, e) ->
-      rho1 ! f = Some (Vfun rhoc B f') ->
-      find_def f B = Some (ft, xs, e) /\ f = f' /\
-      (* eq_env_P (occurs_free_fun_map fm) rho1 (def_funs B B rhoc rhoc) *)
-      preord_env_P_inj cenv PG (occurs_free e \\ FromList xs) i (apply_r sig) (def_funs B B rhoc rhoc) rho2 /\
-      (* sub_map (def_funs B B rhoc rhoc) rho1 /\ *)
-      (* Disjoint _ (bound_var e) (name_in_fundefs B) /\ *)
-      (* Disjoint _ (FromList xs) (name_in_fundefs B) /\ *)
-      (* Disjoint _ S (occurs_free e \\ FromList xs) /\ *)
-      match k with
-      | 0%nat => True
-      | S k => fun_map_inv' k (occurs_free e \\ FromList xs) fm (def_funs B B rhoc rhoc) rho2 i sig
-      end.
-  
-  Lemma fun_map_inv_eq k S fm rho1 rho2 i sig :
-    fun_map_inv k S fm rho1 rho2 i sig = fun_map_inv' k S fm rho1 rho2 i sig.
-  Proof.
-    destruct k; reflexivity.
-  Qed.
-  
-  Lemma fun_map_inv_mon k k' S fm rho1 rho2 i sig :
-    fun_map_inv k S fm rho1 rho2 i sig ->
-    (k' <= k)%nat ->
-    fun_map_inv k' S fm rho1 rho2 i sig.
-  Proof.
-    revert S k fm rho1. induction k' as [k' IHk] using lt_wf_rec1; intros.
-    destruct k'.
-    - unfold fun_map_inv in *. intros. edestruct H; eauto. destructAll.
-      repeat (split; eauto).
-    - destruct k; [ omega | ].
-      intro; intros. edestruct H; eauto. destructAll.
-      split; eauto. split; eauto. split; eauto.
-      rewrite <- fun_map_inv_eq. eapply IHk.
-      omega. rewrite fun_map_inv_eq. eassumption. omega.
-  Qed.
-  
-  Lemma fun_map_inv_antimon k S S' fm rho1 rho2 i sig :
-    fun_map_inv k S fm rho1 rho2 i sig ->
-    S' \subset S ->
-    fun_map_inv k S' fm rho1 rho2 i sig.
-  Proof.
-    intros H1 H2. intro; intros; eauto.
-  Qed.
-
-  Lemma sub_map_set {A} rho x (v : A) :
-    ~ x \in Dom_map rho ->
-    sub_map rho (M.set x v rho).
-  Proof.
-    intros Hnin z1 v1 Hget1. rewrite M.gso; eauto.
-    intros hc. subst. eapply Hnin. eexists; eauto.
-  Qed.
-
-  Lemma sub_map_trans {A} (rho1 rho2 rho3 : M.t A) :
-    sub_map rho1 rho2 ->
-    sub_map rho2 rho3 ->
-    sub_map rho1 rho3.
-  Proof.
-    intros H1 H2 x v Hget. eauto.
-  Qed.
-
-  Lemma sub_map_refl {A} (rho : M.t A) :
-    sub_map rho rho.
-  Proof.
-    intro; intros; eauto.
-  Qed.
-
+    (* [add_fundefs] *)
 
   Lemma add_fundefs_in fm f B ft xs e:
     find_def f B = Some (ft, xs, e) -> 
@@ -369,6 +172,23 @@ Section Inline_correct.
     - reflexivity.
   Qed.
 
+  
+  Lemma Dom_map_add_fundefs fm B :
+    Dom_map (add_fundefs B fm) <--> name_in_fundefs B :|: Dom_map fm.
+  Proof.
+    induction B; simpl; [| now sets ].
+    rewrite Dom_map_set. rewrite IHB. sets.
+  Qed.
+
+
+  (* [occurs_free_fun_map] and [bound_var_fun_map] *)
+  
+  Definition occurs_free_fun_map (fm : fun_map) : Ensemble var :=
+    fun x => exists f ft xs e, fm ! f = Some (ft, xs, e) /\ x \in occurs_free e \\ FromList xs.
+
+  Definition bound_var_fun_map (fm : fun_map) : Ensemble var :=
+    fun x => exists f ft xs e, fm ! f = Some (ft, xs, e) /\ x \in bound_var e :|: FromList xs.
+
 
   Lemma occurs_free_fun_map_get f ft xs e (fm : fun_map) :
     M.get f fm = Some (ft, xs, e) ->
@@ -389,113 +209,17 @@ Section Inline_correct.
       eassumption.
   Qed.
 
-  Lemma funname_in_exp_subset_mut :
-    (forall e, funname_in_exp e \subset bound_var e) /\
-    (forall B, funname_in_fundefs B \subset bound_var_fundefs B).
-  Proof.
-    exp_defs_induction IHe IHl IHB; intros; normalize_bound_var; simpl; sets.
-
-    eapply Union_Included. eapply Union_Included. now sets.
-    eapply Included_trans. eapply name_in_fundefs_bound_var_fundefs. sets.
-    sets.
-  Qed.
-
-  Lemma funname_in_exp_subset :
-    forall e, funname_in_exp e \subset bound_var e.
-  Proof. eapply funname_in_exp_subset_mut. Qed.
-
-  Lemma funname_in_fundefs_subset :
-    forall e, funname_in_fundefs e \subset bound_var_fundefs e.
-  Proof. eapply funname_in_exp_subset_mut. Qed.
-
-
-  Lemma fun_in_fundefs_bound_var_Setminus' e f ft xs B :
-    fun_in_fundefs B (f, ft, xs, e) ->
-    unique_bindings_fundefs B ->
-    bound_var e \\ funname_in_exp e \subset bound_var_fundefs B \\ funname_in_fundefs B \\ name_in_fundefs B.
-  Proof.
-    intros Hin Hun. induction B; [| now inv Hin ].
-    inv Hun. simpl in Hin. inv Hin.
-    - inv H. simpl. normalize_bound_var. rewrite !Setminus_Union_distr. do 2 eapply Included_Union_preserv_r.
-      eapply Included_Union_preserv_l. eapply Included_Setminus.
-      + eapply Union_Disjoint_r. eapply Disjoint_Singleton_r. now intros Hc; inv Hc; eauto.
-        eapply Disjoint_Included_r. eapply name_in_fundefs_bound_var_fundefs. sets.
-      + rewrite <- Setminus_Union. eapply Included_Setminus; [| now sets ].
-        eapply Disjoint_Included_r. eapply funname_in_fundefs_subset. sets.
-    - eapply Included_trans. eapply IHB; eauto.
-      simpl. normalize_bound_var. rewrite !Setminus_Union_distr. do 3 eapply Included_Union_preserv_r.
-      rewrite !Setminus_Union. rewrite <- !Union_assoc. rewrite (Union_commut (funname_in_exp _)). rewrite (Union_commut [set v]).
-      rewrite <- !Union_assoc. rewrite Union_assoc. do 2 rewrite <- Setminus_Union. 
-      eapply Included_Setminus; [| now sets ]. eapply Union_Disjoint_r.
-      eapply Disjoint_Singleton_r. now intros Hc; inv Hc; inv H0; eauto.
-      eapply Disjoint_Included_r. eapply funname_in_exp_subset. sets.
-  Qed.
-
-  Lemma fun_in_fundefs_bound_var_Setminus e f ft xs B :
-    fun_in_fundefs B (f, ft, xs, e) ->
-    unique_bindings_fundefs B ->
-    bound_var e \\ funname_in_exp e \subset bound_var_fundefs B \\ funname_in_fundefs B.
-  Proof.
-    intros Hin Hun. eapply Included_trans. eapply fun_in_fundefs_bound_var_Setminus'. eassumption.
-    eassumption. sets.
-  Qed.
-
-  Lemma fun_in_fundefs_FromList_subset e f ft xs B :
-    fun_in_fundefs B (f, ft, xs, e) ->
-    unique_bindings_fundefs B ->
-    FromList xs \subset bound_var_fundefs B \\ funname_in_fundefs B \\ name_in_fundefs B.
-  Proof.
-    intros Hin Hun. induction B; [| now inv Hin ]. inv Hun. inv Hin.
-    - inv H. simpl. normalize_bound_var. rewrite !Setminus_Union_distr. eapply Included_Union_preserv_r.
-      eapply Included_Union_preserv_l. rewrite !Setminus_Union. eapply Included_Setminus; [| now sets ].
-      eapply Union_Disjoint_r; eapply Union_Disjoint_r.
-      + eapply Disjoint_Included_r. eapply funname_in_exp_subset. sets.
-      + eapply Disjoint_Included_r. eapply funname_in_fundefs_subset. sets.
-      + sets.
-      + eapply Disjoint_Included_r. eapply name_in_fundefs_bound_var_fundefs. sets.
-    - eapply Included_trans. eapply IHB; eauto.
-      simpl. normalize_bound_var. rewrite !Setminus_Union_distr. do 3 eapply Included_Union_preserv_r.
-      rewrite !Setminus_Union. rewrite <- !Union_assoc. rewrite (Union_commut (funname_in_exp _)). rewrite (Union_commut [set v]).
-      rewrite <- !Union_assoc. rewrite Union_assoc. do 2 rewrite <- Setminus_Union. 
-      eapply Included_Setminus; [| now sets ]. eapply Union_Disjoint_r.
-      eapply Disjoint_Singleton_r. now intros Hc; inv Hc; inv H0; eauto.
-      eapply Disjoint_Included_r. eapply funname_in_exp_subset. sets.
-  Qed.
 
   Lemma bound_var_fun_map_get f ft xs e (fm : fun_map) :
     M.get f fm = Some (ft, xs, e) ->
-    bound_var e \\ funname_in_exp e :|: (FromList xs) \subset bound_var_fun_map fm.
+    bound_var e :|: (FromList xs) \subset bound_var_fun_map fm.
   Proof.
     intros Hget z Hin. do 4 eexists. split; eauto.
   Qed.
-
 
   Lemma bound_var_fun_map_add_fundefs_un B fm :
     unique_bindings_fundefs B ->
-    bound_var_fun_map (add_fundefs B fm) \subset (bound_var_fundefs B \\ funname_in_fundefs B \\ name_in_fundefs B) :|: bound_var_fun_map fm.
-  Proof.
-    intros Hun x [z Hin]. destructAll. destruct (Decidable_name_in_fundefs B). destruct (Dec z).
-    - edestruct name_in_fundefs_find_def_is_Some. eassumption. destructAll. erewrite add_fundefs_in in H; [| eassumption ]. inv H.
-      edestruct unique_bindings_fun_in_fundefs. eapply find_def_correct. eassumption. eassumption. destructAll.
-      left.     
-      inv H0.
-      + constructor. eapply fun_in_fundefs_bound_var_Setminus. eapply find_def_correct. eassumption. eassumption. eassumption.
-        inv H8. intros hc. eapply H4; constructor; eauto.
-      + eapply fun_in_fundefs_FromList_subset. eapply find_def_correct. eassumption. eassumption. eassumption.
-    - right. rewrite add_fundefs_not_in in H. do 4 eexists; split; eauto.
-      eassumption.
-  Qed.
-
-  Lemma bound_var_fun_map_get' f ft xs e (fm : fun_map) :
-    M.get f fm = Some (ft, xs, e) ->
-    bound_var e :|: (FromList xs) \subset bound_var_fun_map' fm.
-  Proof.
-    intros Hget z Hin. do 4 eexists. split; eauto.
-  Qed.
-
-  Lemma bound_var_fun_map_add_fundefs_un' B fm :
-    unique_bindings_fundefs B ->
-    bound_var_fun_map' (add_fundefs B fm) \subset (bound_var_fundefs B \\ name_in_fundefs B) :|: bound_var_fun_map' fm.
+    bound_var_fun_map (add_fundefs B fm) \subset (bound_var_fundefs B \\ name_in_fundefs B) :|: bound_var_fun_map fm.
   Proof.
     intros Hun x [z Hin]. destructAll. destruct (Decidable_name_in_fundefs B). destruct (Dec z).
     - edestruct name_in_fundefs_find_def_is_Some. eassumption. destructAll. erewrite add_fundefs_in in H; [| eassumption ]. inv H.
@@ -511,489 +235,6 @@ Section Inline_correct.
       eassumption.
   Qed. 
 
-  (* TODO move *)
-  (* Lemma preord_env_P_inj_set_extend_not_In_P_r_alt S k f rho1 rho2 x y v : *)
-  (*   preord_env_P_inj cenv PG S k f rho1 rho2 -> *)
-  (*   injective_subdomain S (f {x ~> y}) -> *)
-  (*   ~ y \in (image f (Dom_map rho1)) ->             *)
-  (*   preord_env_P_inj cenv PG S k (f {x ~> y}) rho1 (M.set y v rho2). *)
-  (* Proof. *)
-  (*   intros Henv Hnin Hnin' z Hy v' Hget. *)
-  (*   edestruct Henv as [v'' [Hget' Hv]]; eauto. *)
-  (*   eexists; split; eauto.   *)
-  (*   rewrite extend_gso. M.gso. eassumption. *)
-  (*   intros Hc; subst. eapply Hnin'. eexists; eauto. split. eexists; eauto. reflexivity. *)
-  (*   intros Hc. eapply Hnin in Hc. subst. contradiction. *)
-  (* Qed.   *)
-
-  Lemma Dom_map_add_fundefs fm B :
-    Dom_map (add_fundefs B fm) <--> name_in_fundefs B :|: Dom_map fm.
-  Proof.
-    induction B; simpl; [| now sets ].
-    rewrite Dom_map_set. rewrite IHB. sets.
-  Qed.
-
-  
-  Lemma sub_map_def_funs rho B :
-    Disjoint _ (name_in_fundefs B) (Dom_map rho) ->            
-    sub_map rho (def_funs B B rho rho).
-  Proof.
-    intros Hdis x v Hget.
-    rewrite def_funs_neq; eauto.
-    intros Hc. eapply Hdis. constructor. eassumption. eexists. eassumption.
-  Qed.
-
-  Lemma Dom_map_def_funs B rho B' rho' :
-    Dom_map (def_funs B' B rho' rho) <--> name_in_fundefs B :|: Dom_map rho. 
-  Proof.
-    induction B; simpl; sets.
-    rewrite Dom_map_set. rewrite IHB. sets.
-  Qed.
-
-  Lemma Dom_map_sub_map {A : Type} (rho1 rho2 : M.t A) :
-    sub_map rho1 rho2 ->
-    Dom_map rho1 \subset Dom_map rho2.
-  Proof.
-    intros H1 x [y Hin]. eapply H1 in Hin.
-    eexists; eauto.
-  Qed.
-
-  Lemma fun_map_inv_set_not_In_r k S fm rho1 rho2 i sig x x' v' :
-    fun_map_inv k S fm rho1 rho2 i sig ->
-    ~ x \in occurs_free_fun_map fm ->
-    ~ x' \in image (apply_r sig) (occurs_free_fun_map fm) ->
-    fun_map_inv k S fm rho1 (M.set x' v' rho2) i (M.set x x' sig).
-  Proof.
-    revert S fm rho1 rho2 i sig x x' v'. induction k using lt_wf_rec1; intros. intro; intros.
-    edestruct H0; eauto.
-    destructAll. split; [| split; [| split ]]; eauto.
-    - rewrite apply_r_set_f_eq. eapply preord_env_P_inj_set_extend_not_In_P_r. eassumption.
-      + intros Hc. eapply H1. eapply occurs_free_fun_map_get. eassumption. eassumption.
-      + intros Hc. eapply H2. eapply image_monotonic; [| eassumption ].
-        eapply occurs_free_fun_map_get. eassumption.
-    - destruct k; eauto. rewrite <- fun_map_inv_eq in *.
-      eapply H. omega. eassumption.
-      intros hc. eapply H1. eassumption.
-      intros hc. eapply H2. eapply image_monotonic; [| eassumption ]. reflexivity.
-  Qed.
-  
-  Lemma fun_map_inv_set k S fm rho1 rho2 i sig x v x' v' :
-    fun_map_inv k S fm rho1 rho2 i sig ->
-    ~ x \in occurs_free_fun_map fm :|: Dom_map fm ->
-    ~ x' \in image (apply_r sig) (occurs_free_fun_map fm) ->
-    fun_map_inv k (x |: S) fm (M.set x v rho1) (M.set x' v' rho2) i (M.set x x' sig).
-  Proof.
-    intros Hinv Hnin Hnin'. intro; intros.
-    rewrite M.gso in *. 
-    2:{ intros Heq; subst. eapply Hnin. right. eexists; eauto. }
-    inv H.
-    - inv H2. exfalso. eapply Hnin. right. eexists; eauto.
-    - edestruct Hinv; eauto.
-      destructAll. split; [| split; [| split ]]; eauto.
-      + rewrite apply_r_set_f_eq. eapply preord_env_P_inj_set_extend_not_In_P_r. eassumption.
-        intros Hc. eapply Hnin. left. eapply occurs_free_fun_map_get; eauto.
-        intros Hc. eapply Hnin'. eapply image_monotonic; [| eassumption ].
-        eapply occurs_free_fun_map_get. eassumption. 
-      + destruct k; eauto. rewrite <- fun_map_inv_eq in *.
-        eapply fun_map_inv_set_not_In_r. eapply fun_map_inv_antimon. eassumption.
-        * reflexivity.
-        * sets.
-        * sets.
-  Qed.
-  
-  Lemma Dom_map_set_lists {A} xs (vs : list A) rho rho' :
-    set_lists xs vs rho = Some rho' ->
-    Dom_map rho' <--> FromList xs :|: Dom_map rho.
-  Proof.
-    revert vs rho'. induction xs; intros vs rho' Hset.
-    - destruct vs; inv Hset. repeat normalize_sets. reflexivity.
-    - destruct vs; try now inv Hset.
-      simpl in Hset. destruct (set_lists xs vs rho) eqn:Hset1; inv Hset.
-      repeat normalize_sets. rewrite Dom_map_set. rewrite IHxs. now sets.
-      eassumption.
-  Qed.
-
-  Lemma sub_map_set_lists {A} rho rho' xs (vs : list A) :
-    set_lists xs vs rho = Some rho' ->
-    NoDup xs ->
-    Disjoint _ (FromList xs) (Dom_map rho) ->
-    sub_map rho rho'.
-  Proof.
-    revert rho rho' vs; induction xs; intros rho rho' vs Hset; destruct vs; try now inv Hset.
-    simpl in Hset. destruct (set_lists xs vs rho) eqn:Hset'; inv Hset.
-    intros Hnd Hdis. inv Hnd. repeat normalize_sets. eapply sub_map_trans. eapply IHxs. eassumption. eassumption.
-    now sets. eapply sub_map_set. intros Hc. eapply Hdis. constructor. now left.
-    eapply Dom_map_set_lists in Hc; eauto. inv Hc; eauto. exfalso. contradiction.
-  Qed.
-
-
-  Lemma fun_map_inv_sig_extend_Disjoint k S fm rho1 rho2 i sig xs xs' :
-    fun_map_inv k S fm rho1 rho2 i sig ->
-
-    Disjoint _ (FromList xs) (occurs_free_fun_map fm) ->
-    
-    fun_map_inv k S fm rho1 rho2 i (set_list (combine xs xs') sig).
-  Proof.
-    revert S fm rho1 rho2 i sig xs xs'.
-    induction k using lt_wf_rec1; intros S fm rho1 rho2 i sig xs xs' Hfm Hdis1.
-    intro; intros. edestruct Hfm; eauto. destructAll.
-    split; eauto. split; eauto. split.
-    - rewrite apply_r_set_list_f_eq.
-      eapply preord_env_P_inj_extend_lst_not_In_P_r. eassumption.
-      eapply Disjoint_Included_r; [| eapply Hdis1 ].
-      eapply occurs_free_fun_map_get. eassumption.
-    - destruct k; eauto. rewrite <- fun_map_inv_eq in *. eapply H. omega.
-      eassumption.
-      sets.
-  Qed.
-  
-  Lemma fun_map_inv_sig_extend_one_Disjoint k S fm rho1 rho1' rho2 i sig x x' :
-    fun_map_inv k S fm rho1 rho2 i sig ->
-
-    eq_env_P (Complement _ [set x]) rho1 rho1' ->
-    ~ x \in (Dom_map fm) ->
-    ~ x \in (occurs_free_fun_map fm) ->
-    ~ x \in S ->
-                    
-    fun_map_inv k (x |: S) fm rho1' rho2 i (M.set x x' sig).
-  Proof.
-    intros Hfm HeqP Hdis1 Hdis2 Hdis3.
-    intro; intros. inv H. exfalso. inv H2. eapply Hdis1. eexists; eauto.
-    rewrite <- HeqP in H1. 2:{ intros Hc; inv Hc; subst; eauto. }
-    edestruct Hfm; eauto. destructAll.
-    split; eauto. split; eauto. split.
-    - rewrite apply_r_set_f_eq.
-      eapply preord_env_P_inj_extend_not_In_P_r. eassumption.
-      intros Hc. eapply Hdis2. eapply occurs_free_fun_map_get. eassumption.
-      eassumption.
-    - destruct k; eauto. rewrite <- fun_map_inv_eq in *.
-      eapply fun_map_inv_sig_extend_Disjoint with (xs := [x]) (xs' := [x']). eassumption.
-      repeat normalize_sets. eapply Disjoint_Singleton_l.
-      sets.
-  Qed.
-  
-  Lemma fun_map_inv_env_eq_P S k fm rho1 rho2 i sig rho1' rho2' :
-    fun_map_inv k S fm rho1 rho2 i sig ->
-    eq_env_P S rho1 rho1' ->
-    eq_env_P (image (apply_r sig) (occurs_free_fun_map fm)) rho2 rho2' ->    
-    fun_map_inv k S fm rho1' rho2' i sig.
-  Proof.
-    revert S fm rho1 rho2 i sig rho1' rho2'.
-    induction k using lt_wf_rec1; intros S fm rho1 rho2 i sig rho1' rho2' Hfm Heq1 Hsub Heq2.
-    intro; intros. rewrite <- Heq1 in H2; eauto. edestruct Hfm; eauto. destructAll.
-    split; eauto. split; eauto. split.
-    - eapply preord_env_P_inj_eq_env_P.
-      eassumption.
-      now eapply eq_env_P_refl.
-      eapply eq_env_P_antimon. eassumption.
-      eapply image_monotonic. eapply occurs_free_fun_map_get; eauto.
-    - destruct k; eauto. rewrite <- fun_map_inv_eq in *. eapply H. omega.
-      eassumption. eapply eq_env_P_refl. eassumption.
-  Qed.
-
-
-  Lemma eq_env_P_sub_map {A} (rho1 rho2 : M.t A) x:
-    eq_env_P (Complement _ [set x]) rho1 rho2 ->
-    ~ x \in Dom_map rho1 ->
-    sub_map rho1 rho2.
-  Proof.
-    intros Henv Hnin z v Hget.
-    rewrite <- Henv. eassumption. intros Hc. inv Hc.
-    eapply Hnin. eexists; eauto.
-  Qed.
-
-
-  Lemma eq_env_P_set_lists_not_in_P_l  (A : Type) (xs : list var) (vs : list A)
-        (P : Ensemble map_util.M.elt) (rho1 rho1' rho2 : map_util.M.t A) :
-    eq_env_P P rho1 rho2 ->    
-    Disjoint _ P (FromList xs) ->
-    set_lists xs vs rho1 = Some rho1' -> 
-    eq_env_P P rho1' rho2.
-  Proof.
-    intros Heq Hdis Hset x Hin.
-    destruct (Decidable_FromList xs). destruct (Dec x).
-    - exfalso. eapply Hdis. constructor; eauto.
-    - erewrite <- set_lists_not_In; [| eassumption | eassumption ]. eauto.
-  Qed.
-  
-  Lemma fun_map_inv_set_lists k S fm rho1 rho1' rho2 i sig xs vs :
-    fun_map_inv k S fm rho1 rho2 i sig ->
-
-    NoDup xs ->
-    Disjoint _ (FromList xs) (occurs_free_fun_map fm :|: Dom_map fm) ->
-    set_lists xs vs rho1 = Some rho1' ->
-    
-    fun_map_inv k (FromList xs :|: S) fm rho1' rho2 i sig.
-  Proof.
-    revert S fm rho1 rho1' rho2 i sig xs vs.
-    induction k using lt_wf_rec1;
-      intros S fm rho1 rho1' rho2 i sig xs vs Hfm Hnd Hdis1 Hset.
-    intro f; intros.
-    destruct (Decidable_FromList xs). destruct (Dec f).
-    - exfalso. eapply Hdis1. constructor. eassumption. right. eexists; eauto.
-    - inv H0; try contradiction. erewrite <- set_lists_not_In in H2; [| eassumption | eassumption ].
-      edestruct Hfm; eauto.
-  Qed.
-
-
-
-  Lemma preord_env_P_inj_set_lists_not_In_P_r' S k f rho1 rho2 rho2' xs vs :
-    preord_env_P_inj cenv PG S k f rho1 rho2 ->
-    set_lists xs vs rho2 = Some rho2' ->
-    Disjoint _(FromList xs) (image f S) ->
-    preord_env_P_inj cenv PG S k f rho1 rho2'.
-  Proof.
-    intros Henv Hnin Hnin' z Hy v' Hget.
-    edestruct Henv as [v'' [Hget' Hv]]; eauto.
-    eexists; split; eauto. erewrite <- set_lists_not_In. eassumption.
-    eassumption. intros Hc. eapply Hnin'. constructor. eassumption.
-    eapply In_image. eassumption.
-  Qed.
-
-  Lemma fun_map_inv_set_lists_r k S fm rho1 rho2' rho2 i sig xs vs :
-    fun_map_inv k S fm rho1 rho2 i sig ->
-    Disjoint _ (FromList xs) (image (apply_r sig) (occurs_free_fun_map fm)) ->
-
-    set_lists xs vs rho2 = Some rho2' ->
-    
-    fun_map_inv k S fm rho1 rho2' i sig.
-  Proof.
-    revert S fm rho1 rho2' rho2 i sig xs vs.
-    induction k using lt_wf_rec1;
-      intros S fm rho1 rho1' rho2 i sig xs vs Hfm Hdis1 Hset.
-    intro f; intros.
-    edestruct Hfm; eauto. destructAll. split; eauto. split; eauto. split. 
-    + eapply preord_env_P_inj_set_lists_not_In_P_r'. eassumption. eassumption.
-      eapply Disjoint_Included_r; [| eassumption ]. eapply image_monotonic. eapply occurs_free_fun_map_get.
-      eassumption.
-    + destruct k; eauto. rewrite <- fun_map_inv_eq in *.
-      eapply H. omega. eassumption.
-      eapply Disjoint_Included_r; [| eapply Hdis1 ]. reflexivity. eassumption.
-  Qed.
-
-  Lemma fun_map_inv_add_fundefs_Disjoint k S fm rho1 rho2 i sig B1 B2 :
-    fun_map_inv k S fm rho1 rho2 i sig ->
-    
-    Disjoint _ (name_in_fundefs B1) (S :|: occurs_free_fun_map fm) ->
-    Disjoint _ (name_in_fundefs B2) (image (apply_r sig) (occurs_free_fun_map fm)) ->
-
-    fun_map_inv k S (add_fundefs B1 fm) rho1 (def_funs B2 B2 rho2 rho2) i
-                (set_list (combine (all_fun_name B1) (all_fun_name B2)) sig).
-  Proof.
-    revert S fm rho1 rho2 i sig B1 B2; induction k using lt_wf_rec1; intros.
-    intro; intros. rewrite add_fundefs_not_in in H4.
-    edestruct H0; eauto. destructAll.
-    repeat (split; [ now eauto |]). split.
-    - eapply preord_env_P_inj_def_funs_neq_r.
-      rewrite apply_r_set_list_f_eq. eapply preord_env_P_inj_extend_lst_not_In_P_r.
-      eassumption. rewrite <- Same_set_all_fun_name.
-      eapply Disjoint_Included_r; [| eapply H1 ]. eapply Included_Union_preserv_r.
-      eapply occurs_free_fun_map_get. eassumption.
-      
-      rewrite apply_r_set_list_f_eq. eapply Disjoint_Included_l.
-      intros x Hc. destruct Hc. destructAll.
-      rewrite extend_lst_gso. eapply In_image. eassumption.
-      rewrite <- Same_set_all_fun_name. intros Hc. eapply H1. constructor. eassumption. right.
-      eapply occurs_free_fun_map_get. eassumption. eassumption.
-      eapply Disjoint_sym. eapply Disjoint_Included_r; [| eassumption ]. eapply image_monotonic.
-      eapply occurs_free_fun_map_get. eassumption.
-    - destruct k; eauto. rewrite <- fun_map_inv_eq in *. eapply H.
-      + omega.
-      + eassumption.
-      + eapply Union_Disjoint_r; [| sets ].
-        eapply Disjoint_Included_r; [| eassumption ]. eapply Included_Union_preserv_r.
-      eapply occurs_free_fun_map_get. eassumption.
-      + sets.
-    - intros Hc. eapply H1. constructor. eassumption. now left ; eauto.
-  Qed.
-
-  
-  Lemma name_in_fundefs_funname_in_fundefs_Disjoint B1 : 
-    unique_bindings_fundefs B1 ->
-    Disjoint _ (name_in_fundefs B1) (funname_in_fundefs B1).
-  Proof.
-    induction B1; intros Hun.
-    - inv Hun. simpl. eapply Union_Disjoint_r; eapply Union_Disjoint_l.
-      + eapply Disjoint_Included_r. eapply funname_in_exp_subset. sets.
-      + eapply Disjoint_sym. eapply Disjoint_Included.
-        eapply name_in_fundefs_bound_var_fundefs. eapply funname_in_exp_subset. eassumption. 
-      + eapply Disjoint_Included_r. eapply funname_in_fundefs_subset. sets.
-      + eauto.
-    - sets.
-  Qed.
-        
-  Lemma fun_map_inv_def_funs k S fm rho1 rho2 i sig B1 B2 :
-    fun_map_inv k S fm rho1 rho2 i sig ->
-    
-    preord_env_P_inj cenv PG (name_in_fundefs B1 :|: occurs_free_fundefs B1) i
-                     (apply_r (set_list (combine (all_fun_name B1) (all_fun_name B2)) sig))
-                     (def_funs B1 B1 rho1 rho1) (def_funs B2 B2 rho2 rho2) ->
-
-    unique_bindings_fundefs B1 ->
-    occurs_free_fundefs B1 \subset S ->
-    
-    Disjoint _ (name_in_fundefs B1) (S :|: occurs_free_fun_map fm) ->
-    Disjoint _ (name_in_fundefs B2) (image (apply_r sig) (occurs_free_fun_map fm)) ->        
-    
-    fun_map_inv k (name_in_fundefs B1 :|: S) (add_fundefs B1 fm) (def_funs B1 B1 rho1 rho1) (def_funs B2 B2 rho2 rho2) i
-                (set_list (combine (all_fun_name B1) (all_fun_name B2)) sig).
-  Proof.
-    revert S fm rho1 rho2 i sig B1 B2. induction k as [k IHk] using lt_wf_rec1.
-    intros S fm rho1 rho2 i sig B1 B2 Hf Hrel Hun Hsub Hdis Hdis'.
-    intros f ft xs e rhoc B' f' HSin Heq1 Heq2.
-    destruct (Decidable_name_in_fundefs B1) as [Dec]. destruct (Dec f).
-    - rewrite def_funs_eq in Heq2; eauto. inv Heq2.
-      edestruct name_in_fundefs_find_def_is_Some. eassumption. destructAll.
-      erewrite add_fundefs_in in Heq1; [| eassumption ]. inv Heq1. split; eauto.
-      split; eauto. split.
-      + eapply preord_env_P_inj_antimon. eassumption. eapply Setminus_Included_Included_Union.
-        eapply Included_trans. eapply occurs_free_in_fun. eapply find_def_correct. eassumption. sets.
-      (* + eapply find_def_correct in H. assert (H' := H). eapply unique_bindings_fun_in_fundefs in H; eauto. destructAll. *)
-      (*   eassumption. *)
-      (* + eapply find_def_correct in H. assert (H' := H). eapply unique_bindings_fun_in_fundefs in H; eauto. destructAll. *)
-      (*   eassumption. *)
-      + destruct k; eauto. rewrite <- fun_map_inv_eq. eapply fun_map_inv_antimon. eapply IHk.
-        omega. eapply fun_map_inv_mon. eassumption. omega. eassumption. eassumption.
-        eassumption. now sets. now sets. eapply Setminus_Included_Included_Union. 
-        eapply Included_trans. eapply occurs_free_in_fun. eapply find_def_correct. eassumption.
-        sets.
-    - rewrite def_funs_neq in Heq2; eauto.
-      rewrite add_fundefs_not_in in Heq1; [| eassumption ]. inv HSin. contradiction.
-      edestruct Hf. eassumption. eassumption. eassumption. destructAll. split; eauto. split; eauto. split.
-      + eapply preord_env_P_inj_def_funs_neq_r.
-        rewrite apply_r_set_list_f_eq. eapply preord_env_P_inj_extend_lst_not_In_P_r.
-        eassumption.
-        * rewrite <- Same_set_all_fun_name.
-          eapply Disjoint_Included; [| | eapply Hdis ]. eapply Included_Union_preserv_r.
-          eapply occurs_free_fun_map_get. eassumption. reflexivity. 
-        * rewrite apply_r_set_list_f_eq. eapply Disjoint_Included_l. 
-          intros x Hc. destruct Hc. destructAll.
-          rewrite extend_lst_gso. eapply In_image. eassumption.
-          rewrite <- Same_set_all_fun_name. intros Hc. eapply Hdis. constructor.
-          eassumption. right.
-          eapply occurs_free_fun_map_get. eassumption. eassumption.
-          eapply Disjoint_sym. eapply Disjoint_Included_r; [| eassumption ]. apply image_monotonic.
-          eapply occurs_free_fun_map_get. eassumption.
-      + destruct k; eauto. rewrite <- fun_map_inv_eq in *.
-        eapply fun_map_inv_add_fundefs_Disjoint; try eassumption.
-        * eapply Union_Disjoint_r; [| sets ].
-          eapply Disjoint_Included_r; [| eassumption ]. eapply Included_Union_preserv_r.
-          eapply occurs_free_fun_map_get. eassumption. 
-  Qed.
-
-  Lemma fun_in_fundefs_funname_in_exp f ft xs e B :
-    (f, ft, xs, e) \infun_in_fundefs B ->
-    funname_in_exp e \subset funname_in_fundefs B.
-  Proof.
-    induction B; intros Hin; inv Hin.
-    + inv H. sets.
-    + simpl. eapply Included_Union_preserv_r. eauto.
-  Qed.
-  
-  Definition funname_fun_map (fm : fun_map) : Ensemble var :=
-    fun x => exists f ft xs e, fm ! f = Some (ft, xs, e) /\ x \in funname_in_exp e.
-
-  Lemma funname_fun_map_fun_map_get f ft xs e (fm : fun_map) :
-    M.get f fm = Some (ft, xs, e) ->
-    funname_in_exp e \subset funname_fun_map fm.
-  Proof.
-    intros Hget z Hin. do 4 eexists. split; eauto.
-  Qed.
-  
-
-  Lemma funname_fun_map_add_fundefs B fm :
-    funname_fun_map (add_fundefs B fm) \subset (funname_in_fundefs B) :|: funname_fun_map fm.
-  Proof.
-    intros x [z Hin]. destructAll. destruct (Decidable_name_in_fundefs B). destruct (Dec z).
-    - edestruct name_in_fundefs_find_def_is_Some. eassumption. destructAll.
-      erewrite add_fundefs_in in H; [| eassumption ]. inv H.
-      left. eapply fun_in_fundefs_funname_in_exp. eapply find_def_correct. eassumption. eassumption.
-    - right. rewrite add_fundefs_not_in in H. do 4 eexists; split; eauto.
-      eassumption.
-  Qed.
-  
-  Definition fun_map_vars (fm : fun_map) (F : Ensemble var) (sig : subst) :=
-    forall f ft xs e,
-      fm ! f = Some (ft, xs, e) ->
-      unique_bindings e /\
-      NoDup xs /\
-
-      Disjoint _ (bound_var e) (FromList xs :|: occurs_free e) /\
-
-      Disjoint _ (bound_var e \\ funname_in_exp e) (Dom_map fm :|: funname_fun_map fm) /\
-    
-      Disjoint _ (bound_var e :|: FromList xs) (occurs_free_fun_map (M.remove f fm)) /\
-      Disjoint _ (bound_var e :|: occurs_free e) (bound_var_fun_map' (M.remove f fm)) /\
-      
-      Disjoint _ (FromList xs) (Dom_map fm) /\
-      Disjoint _ (funname_in_exp e) (bound_var_fun_map fm) /\
-      
-      Disjoint _ F (bound_var e :|: image (apply_r sig) (occurs_free e \\ FromList xs)).
-
-  Lemma fun_map_vars_antimon fm F F' sig :
-    fun_map_vars fm F sig ->
-    F' \subset F ->
-    fun_map_vars fm F' sig.
-  Proof.
-    intros Hfm Hsub; intro; intros. eapply Hfm in H. destructAll.
-    do 6 (split; eauto). sets.
-  Qed.
-
-  Instance fm_map_vars_Proper fm : Proper (Same_set _ ==> eq ==> iff) (fun_map_vars fm).
-  Proof.
-    repeat (intro; intros). subst. split; intros.
-    intro; intros. eapply H0 in H1. rewrite H in H1. eauto.
-    intro; intros. eapply H0 in H1. rewrite <- H in H1. eauto.
-  Qed.
-
-
-  Lemma fun_map_vars_set fm F sig x v :
-    fun_map_vars fm F sig ->
-    fun_map_vars fm (F \\ [set v]) (M.set x v sig).
-  Proof.
-    intros Hfm; intro; intros. eapply Hfm in H. destructAll.
-    do 8 (split; eauto). eapply Union_Disjoint_r. now sets.
-    eapply Disjoint_Included_r. eapply image_apply_r_set.
-    eapply Union_Disjoint_r. now sets. now xsets.
-  Qed.
-  
-  Lemma fun_map_vars_set_list fm F sig xs vs :
-    fun_map_vars fm F sig ->
-    fun_map_vars fm (F \\ FromList vs) (set_list (combine xs vs) sig).
-  Proof.
-    revert F vs sig. induction xs; intros F vs sig.
-    - simpl. intros Hin. eapply fun_map_vars_antimon. eassumption.
-      now sets.
-    - destruct vs; simpl.
-      + intros Hf. eapply fun_map_vars_antimon. eassumption. sets.
-      + intros Hfm. simpl. repeat normalize_sets. rewrite Union_commut.
-        rewrite <- Setminus_Union. eapply fun_map_vars_set. 
-        simpl. eapply IHxs; eauto.
-  Qed.
-
-  Lemma apply_r_list_eq xs ys sig :
-    NoDup xs ->
-    length xs = length ys ->
-    apply_r_list (set_list (combine xs ys) sig) xs = ys.
-  Proof.
-    revert ys sig; induction xs; intros ys sig Hnd Hlen.
-    - simpl. destruct ys; eauto. inv Hlen.
-    - destruct ys; inv Hlen. inv Hnd.
-      simpl. unfold apply_r. rewrite M.gss. f_equal.
-      erewrite eq_P_apply_r_list. eapply IHxs. eassumption. eassumption.
-      eapply eq_env_P_set_not_in_P_l. eapply eq_env_P_refl. eassumption.
-  Qed.
-
-  Lemma NoDup_all_fun_name B :
-    unique_bindings_fundefs B ->
-    NoDup (all_fun_name B).
-  Proof.
-    induction B; intros Hc; inv Hc.
-    - simpl. constructor; eauto.
-      intros Hc. eapply Same_set_all_fun_name in Hc. eapply H5.
-      eapply name_in_fundefs_bound_var_fundefs. eassumption.
-    - constructor.
-  Qed.
 
   Lemma occurs_free_fun_map_remove_add_fundefs B f fm :
     occurs_free_fun_map (M.remove f (add_fundefs B fm)) \subset occurs_free_fundefs B :|: name_in_fundefs B :|: occurs_free_fun_map (M.remove f fm).
@@ -1020,8 +261,8 @@ Section Inline_correct.
 
   Lemma bound_var_fun_map_remove_add_fundefs_un' (B : fundefs) (fm : fun_map) f :
     unique_bindings_fundefs B ->
-    bound_var_fun_map' (M.remove f (add_fundefs B fm)) \subset
-    bound_var_fundefs B \\ name_in_fundefs B :|: bound_var_fun_map' (M.remove f fm).
+    bound_var_fun_map (M.remove f (add_fundefs B fm)) \subset
+    bound_var_fundefs B \\ name_in_fundefs B :|: bound_var_fun_map (M.remove f fm).
   Proof.
     intros Hun x [z Hin]. destructAll. destruct (peq f z); subst.
     - rewrite M.grs in H. inv H.
@@ -1040,11 +281,11 @@ Section Inline_correct.
         rewrite M.gro; now eauto. eassumption.
   Qed. 
 
-  Lemma bound_var_fun_map_remove_add_fundefs_un'' (B : fundefs) (fm : fun_map) f ft xs e:
+  Lemma bound_var_fun_map_remove_add_fundefs_un (B : fundefs) (fm : fun_map) f ft xs e:
     unique_bindings_fundefs B ->
     find_def f B = Some (ft, xs, e) ->
-    bound_var_fun_map' (M.remove f (add_fundefs B fm)) \subset
-    bound_var_fundefs B \\ name_in_fundefs B \\ bound_var e \\ FromList xs :|: bound_var_fun_map' (M.remove f fm).
+    bound_var_fun_map (M.remove f (add_fundefs B fm)) \subset
+    bound_var_fundefs B \\ name_in_fundefs B \\ bound_var e \\ FromList xs :|: bound_var_fun_map (M.remove f fm).
   Proof.
     induction B.
     - intros Hun Hfind. inv Hun. destruct (peq f v); subst.
@@ -1090,7 +331,7 @@ Section Inline_correct.
                 eapply fun_in_fundefs_bound_var_fundefs. eapply find_def_correct. eassumption. now eauto.
                 eassumption.
           -- rewrite M.gso in H.         
-             assert (Hin' : x \in bound_var_fun_map' (M.remove f (add_fundefs B fm))).
+             assert (Hin' : x \in bound_var_fun_map (M.remove f (add_fundefs B fm))).
              { do 4 eexists. split. rewrite M.gro. eassumption. now eauto. eassumption. }
              eapply Hfind in Hin'. inv Hin'; [| now eauto ]. left. inv H1. inv H2. inv H1. 
              constructor. constructor. constructor. eauto.
@@ -1102,30 +343,534 @@ Section Inline_correct.
   Qed. 
 
   Lemma  bound_var_fun_map_remove f fm :
-    bound_var_fun_map' (M.remove f fm) \subset bound_var_fun_map' fm.
+    bound_var_fun_map (M.remove f fm) \subset bound_var_fun_map fm.
   Proof.
     intros x [z Hin]. destructAll. destruct (peq f z); subst.
     - rewrite M.grs in H. inv H.
     - rewrite M.gro in H; eauto. do 4 eexists; split; eauto.
   Qed.
 
+
+  Lemma occurs_free_fun_map_remove' f f' fm :
+    occurs_free_fun_map (M.remove f (M.remove f' fm)) \subset occurs_free_fun_map (M.remove f fm).
+  Proof.
+    intros x [z Hin]. destructAll. destruct (peq f z); subst.
+    - rewrite M.grs in H. inv H.
+    - rewrite M.gro in H; eauto.
+      destruct (peq f' z); subst. rewrite M.grs in H. inv H.
+      rewrite M.gro in H; eauto. 
+      do 4 eexists; split; eauto. rewrite M.gro. eassumption. eauto. 
+  Qed.
+
+
+  Lemma bound_var_fun_map_remove' f f' fm :
+    bound_var_fun_map (M.remove f (M.remove f' fm)) \subset bound_var_fun_map (M.remove f fm).
+  Proof.
+    intros x [z Hin]. destructAll. destruct (peq f z); subst.
+    - rewrite M.grs in H. inv H.
+    - rewrite M.gro in H; eauto.
+      destruct (peq f' z); subst. rewrite M.grs in H. inv H.
+      rewrite M.gro in H; eauto. 
+      do 4 eexists; split; eauto. rewrite M.gro. eassumption. eauto. 
+  Qed.
+
+  (* Various lemmas *)
+
+  Lemma sub_map_def_funs rho B :
+    Disjoint _ (name_in_fundefs B) (Dom_map rho) ->            
+    sub_map rho (def_funs B B rho rho).
+  Proof.
+    intros Hdis x v Hget.
+    rewrite def_funs_neq; eauto.
+    intros Hc. eapply Hdis. constructor. eassumption. eexists. eassumption.
+  Qed.
+  
+  Lemma Dom_map_def_funs B rho B' rho' :
+    Dom_map (def_funs B' B rho' rho) <--> name_in_fundefs B :|: Dom_map rho. 
+  Proof.
+    induction B; simpl; sets.
+    rewrite Dom_map_set. rewrite IHB. sets.
+  Qed.
+
+  (* TODO move *)
+  Lemma preord_env_P_inj_set_lists_not_In_P_r' S k f rho1 rho2 rho2' xs vs :
+    preord_env_P_inj cenv PG S k f rho1 rho2 ->
+    set_lists xs vs rho2 = Some rho2' ->
+    Disjoint _(FromList xs) (image f S) ->
+    preord_env_P_inj cenv PG S k f rho1 rho2'.
+  Proof.
+    intros Henv Hnin Hnin' z Hy v' Hget.
+    edestruct Henv as [v'' [Hget' Hv]]; eauto.
+    eexists; split; eauto. erewrite <- set_lists_not_In. eassumption.
+    eassumption. intros Hc. eapply Hnin'. constructor. eassumption.
+    eapply In_image. eassumption.
+  Qed.
+
+  Lemma NoDup_all_fun_name B :
+    unique_bindings_fundefs B ->
+    NoDup (all_fun_name B).
+  Proof.
+    induction B; intros Hc; inv Hc.
+    - simpl. constructor; eauto.
+      intros Hc. eapply Same_set_all_fun_name in Hc. eapply H5.
+      eapply name_in_fundefs_bound_var_fundefs. eassumption.
+    - constructor.
+  Qed.
+
+  (* [Fun_map_inv] *)
+  
+  Fixpoint fun_map_inv' (k : nat) (S : Ensemble var) (fm : fun_map) (rho1 rho2 : env) (i : nat) (sig : subst) : Prop :=
+    forall f ft xs e rhoc B f',
+      f \in S ->
+      fm ! f = Some (ft, xs, e) ->
+      rho1 ! f = Some (Vfun rhoc B f') ->
+      find_def f B = Some (ft, xs, e) /\ f = f' /\
+      preord_env_P_inj cenv PG (occurs_free e \\ FromList xs) i (apply_r sig) (def_funs B B rhoc rhoc) rho2 /\
+      match k with
+      | 0%nat => True
+      | S k => fun_map_inv' k (occurs_free e \\ FromList xs) fm (def_funs B B rhoc rhoc) rho2 i sig
+      end.
+
+  Definition fun_map_inv (k : nat) (S : Ensemble var) (fm : fun_map) (rho1 rho2 : env) (i : nat) (sig : subst) : Prop :=
+    forall f ft xs e rhoc B f',
+      f \in S ->
+      fm ! f = Some (ft, xs, e) ->
+      rho1 ! f = Some (Vfun rhoc B f') ->
+      find_def f B = Some (ft, xs, e) /\ f = f' /\
+      preord_env_P_inj cenv PG (occurs_free e \\ FromList xs) i (apply_r sig) (def_funs B B rhoc rhoc) rho2 /\
+      match k with
+      | 0%nat => True
+      | S k => fun_map_inv' k (occurs_free e \\ FromList xs) fm (def_funs B B rhoc rhoc) rho2 i sig
+      end.
+  
+  Lemma fun_map_inv_eq k S fm rho1 rho2 i sig :
+    fun_map_inv k S fm rho1 rho2 i sig = fun_map_inv' k S fm rho1 rho2 i sig.
+  Proof.
+    destruct k; reflexivity.
+  Qed.
+  
+  Lemma fun_map_inv_mon k k' S fm rho1 rho2 i sig :
+    fun_map_inv k S fm rho1 rho2 i sig ->
+    (k' <= k)%nat ->
+    fun_map_inv k' S fm rho1 rho2 i sig.
+  Proof.
+    revert S k fm rho1. induction k' as [k' IHk] using lt_wf_rec1; intros.
+    destruct k'.
+    - unfold fun_map_inv in *. intros. edestruct H; eauto. destructAll.
+      repeat (split; eauto).
+    - destruct k; [ omega | ].
+      intro; intros. edestruct H; eauto. destructAll.
+      split; eauto. split; eauto. split; eauto.
+      rewrite <- fun_map_inv_eq. eapply IHk.
+      omega. rewrite fun_map_inv_eq. eassumption. omega.
+  Qed.
+  
+  Lemma fun_map_inv_antimon k S S' fm rho1 rho2 i sig :
+    fun_map_inv k S fm rho1 rho2 i sig ->
+    S' \subset S ->
+    fun_map_inv k S' fm rho1 rho2 i sig.
+  Proof.
+    intros H1 H2. intro; intros; eauto.
+  Qed.
+
+
+  Lemma fun_map_inv_set_not_In_r k S fm rho1 rho2 i sig x x' v' :
+    fun_map_inv k S fm rho1 rho2 i sig ->
+    ~ x \in occurs_free_fun_map fm ->
+    ~ x' \in image (apply_r sig) (occurs_free_fun_map fm) ->
+    fun_map_inv k S fm rho1 (M.set x' v' rho2) i (M.set x x' sig).
+  Proof.
+    revert S fm rho1 rho2 i sig x x' v'. induction k using lt_wf_rec1; intros. intro; intros.
+    edestruct H0; eauto.
+    destructAll. split; [| split; [| split ]]; eauto.
+    - rewrite apply_r_set_f_eq. eapply preord_env_P_inj_set_extend_not_In_P_r. eassumption.
+      + intros Hc. eapply H1. eapply occurs_free_fun_map_get. eassumption. eassumption.
+      + intros Hc. eapply H2. eapply image_monotonic; [| eassumption ].
+        eapply occurs_free_fun_map_get. eassumption.
+    - destruct k; eauto. rewrite <- fun_map_inv_eq in *.
+      eapply H. omega. eassumption.
+      intros hc. eapply H1. eassumption.
+      intros hc. eapply H2. eapply image_monotonic; [| eassumption ]. reflexivity.
+  Qed.
+  
+  Lemma fun_map_inv_set k S fm rho1 rho2 i sig x v x' v' :
+    fun_map_inv k S fm rho1 rho2 i sig ->
+    ~ x \in occurs_free_fun_map fm :|: Dom_map fm ->
+    ~ x' \in image (apply_r sig) (occurs_free_fun_map fm) ->
+    fun_map_inv k (x |: S) fm (M.set x v rho1) (M.set x' v' rho2) i (M.set x x' sig).
+  Proof.
+    intros Hinv Hnin Hnin'. intro; intros.
+    rewrite M.gso in *. 
+    2:{ intros Heq; subst. eapply Hnin. right. eexists; eauto. }
+    inv H.
+    - inv H2. exfalso. eapply Hnin. right. eexists; eauto.
+    - edestruct Hinv; eauto.
+      destructAll. split; [| split; [| split ]]; eauto.
+      + rewrite apply_r_set_f_eq. eapply preord_env_P_inj_set_extend_not_In_P_r. eassumption.
+        intros Hc. eapply Hnin. left. eapply occurs_free_fun_map_get; eauto.
+        intros Hc. eapply Hnin'. eapply image_monotonic; [| eassumption ].
+        eapply occurs_free_fun_map_get. eassumption. 
+      + destruct k; eauto. rewrite <- fun_map_inv_eq in *.
+        eapply fun_map_inv_set_not_In_r. eapply fun_map_inv_antimon. eassumption.
+        * reflexivity.
+        * sets.
+        * sets.
+  Qed.
+  
+  Lemma fun_map_inv_sig_extend_Disjoint k S fm rho1 rho2 i sig xs xs' :
+    fun_map_inv k S fm rho1 rho2 i sig ->
+
+    Disjoint _ (FromList xs) (occurs_free_fun_map fm) ->
+    
+    fun_map_inv k S fm rho1 rho2 i (set_list (combine xs xs') sig).
+  Proof.
+    revert S fm rho1 rho2 i sig xs xs'.
+    induction k using lt_wf_rec1; intros S fm rho1 rho2 i sig xs xs' Hfm Hdis1.
+    intro; intros. edestruct Hfm; eauto. destructAll.
+    split; eauto. split; eauto. split.
+    - rewrite apply_r_set_list_f_eq.
+      eapply preord_env_P_inj_extend_lst_not_In_P_r. eassumption.
+      eapply Disjoint_Included_r; [| eapply Hdis1 ].
+      eapply occurs_free_fun_map_get. eassumption.
+    - destruct k; eauto. rewrite <- fun_map_inv_eq in *. eapply H. omega.
+      eassumption.
+      sets.
+  Qed.
+
+  
+  Lemma fun_map_inv_sig_extend_one_Disjoint k S fm rho1 rho1' rho2 i sig x x' :
+    fun_map_inv k S fm rho1 rho2 i sig ->
+
+    eq_env_P (Complement _ [set x]) rho1 rho1' ->
+    ~ x \in (Dom_map fm) ->
+    ~ x \in (occurs_free_fun_map fm) ->
+    ~ x \in S ->
+                    
+    fun_map_inv k (x |: S) fm rho1' rho2 i (M.set x x' sig).
+  Proof.
+    intros Hfm HeqP Hdis1 Hdis2 Hdis3.
+    intro; intros. inv H. exfalso. inv H2. eapply Hdis1. eexists; eauto.
+    rewrite <- HeqP in H1. 2:{ intros Hc; inv Hc; subst; eauto. }
+    edestruct Hfm; eauto. destructAll.
+    split; eauto. split; eauto. split.
+    - rewrite apply_r_set_f_eq.
+      eapply preord_env_P_inj_extend_not_In_P_r. eassumption.
+      intros Hc. eapply Hdis2. eapply occurs_free_fun_map_get. eassumption.
+      eassumption.
+    - destruct k; eauto. rewrite <- fun_map_inv_eq in *.
+      eapply fun_map_inv_sig_extend_Disjoint with (xs := [x]) (xs' := [x']). eassumption.
+      repeat normalize_sets. eapply Disjoint_Singleton_l.
+      sets.
+  Qed.
+  
+  Lemma fun_map_inv_env_eq_P S k fm rho1 rho2 i sig rho1' rho2' :
+    fun_map_inv k S fm rho1 rho2 i sig ->
+    eq_env_P S rho1 rho1' ->
+    eq_env_P (image (apply_r sig) (occurs_free_fun_map fm)) rho2 rho2' ->    
+    fun_map_inv k S fm rho1' rho2' i sig.
+  Proof.
+    revert S fm rho1 rho2 i sig rho1' rho2'.
+    induction k using lt_wf_rec1; intros S fm rho1 rho2 i sig rho1' rho2' Hfm Heq1 Hsub Heq2.
+    intro; intros. rewrite <- Heq1 in H2; eauto. edestruct Hfm; eauto. destructAll.
+    split; eauto. split; eauto. split.
+    - eapply preord_env_P_inj_eq_env_P.
+      eassumption.
+      now eapply eq_env_P_refl.
+      eapply eq_env_P_antimon. eassumption.
+      eapply image_monotonic. eapply occurs_free_fun_map_get; eauto.
+    - destruct k; eauto. rewrite <- fun_map_inv_eq in *. eapply H. omega.
+      eassumption. eapply eq_env_P_refl. eassumption.
+  Qed.
+
+  
+  Lemma fun_map_inv_set_lists k S fm rho1 rho1' rho2 i sig xs vs :
+    fun_map_inv k S fm rho1 rho2 i sig ->
+
+    NoDup xs ->
+    Disjoint _ (FromList xs) (occurs_free_fun_map fm :|: Dom_map fm) ->
+    set_lists xs vs rho1 = Some rho1' ->
+    
+    fun_map_inv k (FromList xs :|: S) fm rho1' rho2 i sig.
+  Proof.
+    revert S fm rho1 rho1' rho2 i sig xs vs.
+    induction k using lt_wf_rec1;
+      intros S fm rho1 rho1' rho2 i sig xs vs Hfm Hnd Hdis1 Hset.
+    intro f; intros.
+    destruct (Decidable_FromList xs). destruct (Dec f).
+    - exfalso. eapply Hdis1. constructor. eassumption. right. eexists; eauto.
+    - inv H0; try contradiction. erewrite <- set_lists_not_In in H2; [| eassumption | eassumption ].
+      edestruct Hfm; eauto.
+  Qed.
+
+
+  Lemma fun_map_inv_set_lists_r k S fm rho1 rho2' rho2 i sig xs vs :
+    fun_map_inv k S fm rho1 rho2 i sig ->
+    Disjoint _ (FromList xs) (image (apply_r sig) (occurs_free_fun_map fm)) ->
+
+    set_lists xs vs rho2 = Some rho2' ->
+    
+    fun_map_inv k S fm rho1 rho2' i sig.
+  Proof.
+    revert S fm rho1 rho2' rho2 i sig xs vs.
+    induction k using lt_wf_rec1;
+      intros S fm rho1 rho1' rho2 i sig xs vs Hfm Hdis1 Hset.
+    intro f; intros.
+    edestruct Hfm; eauto. destructAll. split; eauto. split; eauto. split. 
+    + eapply preord_env_P_inj_set_lists_not_In_P_r'. eassumption. eassumption.
+      eapply Disjoint_Included_r; [| eassumption ]. eapply image_monotonic. eapply occurs_free_fun_map_get.
+      eassumption.
+    + destruct k; eauto. rewrite <- fun_map_inv_eq in *.
+      eapply H. omega. eassumption.
+      eapply Disjoint_Included_r; [| eapply Hdis1 ]. reflexivity. eassumption.
+  Qed.
+
+  Lemma fun_map_inv_def_funs_Disjoint k S fm rho1 rho2 i sig B1 B2 :
+    fun_map_inv k S fm rho1 rho2 i sig ->
+    
+    Disjoint _ (name_in_fundefs B1) (S :|: occurs_free_fun_map fm) ->
+    Disjoint _ (name_in_fundefs B2) (image (apply_r sig) (occurs_free_fun_map fm)) ->
+
+    fun_map_inv k S fm rho1 (def_funs B2 B2 rho2 rho2) i
+                (set_list (combine (all_fun_name B1) (all_fun_name B2)) sig).
+  Proof.
+    revert S fm rho1 rho2 i sig B1 B2; induction k using lt_wf_rec1; intros.
+    intro; intros.
+    edestruct H0; eauto. destructAll.
+    repeat (split; [ now eauto |]). split.
+    - eapply preord_env_P_inj_def_funs_neq_r.
+      rewrite apply_r_set_list_f_eq. eapply preord_env_P_inj_extend_lst_not_In_P_r.
+      eassumption. rewrite <- Same_set_all_fun_name.
+      eapply Disjoint_Included_r; [| eapply H1 ]. eapply Included_Union_preserv_r.
+      eapply occurs_free_fun_map_get. eassumption.
+      
+      rewrite apply_r_set_list_f_eq. eapply Disjoint_Included_l.
+      intros x Hc. destruct Hc. destructAll.
+      rewrite extend_lst_gso. eapply In_image. eassumption.
+      rewrite <- Same_set_all_fun_name. intros Hc. eapply H1. constructor. eassumption. right.
+      eapply occurs_free_fun_map_get. eassumption. eassumption.
+      eapply Disjoint_sym. eapply Disjoint_Included_r; [| eassumption ]. eapply image_monotonic.
+      eapply occurs_free_fun_map_get. eassumption.
+    - destruct k; eauto. rewrite <- fun_map_inv_eq in *. eapply H.
+      + omega.
+      + eassumption.
+      + eapply Union_Disjoint_r; [| sets ].
+        eapply Disjoint_Included_r; [| eassumption ]. eapply Included_Union_preserv_r.
+      eapply occurs_free_fun_map_get. eassumption.
+      + sets.
+  Qed.
+
+  Lemma fun_map_inv_add_fundefs k S fm rho1 rho2 i sig B1 (* B2 *) :
+    fun_map_inv k S fm rho1 rho2 i sig ->
+    
+    Disjoint _ (name_in_fundefs B1) (S :|: occurs_free_fun_map fm) ->
+
+    fun_map_inv k S (add_fundefs B1 fm) rho1 rho2 i sig.
+  Proof.
+    revert S fm rho1 rho2 i sig B1 (* B2 *); induction k using lt_wf_rec1; intros.
+    intro; intros. rewrite add_fundefs_not_in in H3.
+    2:{ intros Hc. eapply H1. constructor. eassumption. left. eassumption. }
+    edestruct H0; eauto. destructAll.
+    repeat (split; [ now eauto |]).
+    destruct k; eauto. rewrite <- fun_map_inv_eq in *. eapply H.
+    + omega.
+    + eassumption.
+    + eapply Union_Disjoint_r; [| sets ].
+      eapply Disjoint_Included_r; [| eassumption ]. eapply Included_Union_preserv_r.
+      eapply occurs_free_fun_map_get. eassumption.
+  Qed.
+        
+  Lemma fun_map_inv_def_funs_add_fundefs k S fm rho1 rho2 i sig B1 B2 :
+    fun_map_inv k S fm rho1 rho2 i sig ->
+    
+    preord_env_P_inj cenv PG (name_in_fundefs B1 :|: occurs_free_fundefs B1) i
+                     (apply_r (set_list (combine (all_fun_name B1) (all_fun_name B2)) sig))
+                     (def_funs B1 B1 rho1 rho1) (def_funs B2 B2 rho2 rho2) ->
+
+    unique_bindings_fundefs B1 ->
+    occurs_free_fundefs B1 \subset S ->
+    
+    Disjoint _ (name_in_fundefs B1) (S :|: occurs_free_fun_map fm) ->
+    Disjoint _ (name_in_fundefs B2) (image (apply_r sig) (occurs_free_fun_map fm)) ->        
+    
+    fun_map_inv k (name_in_fundefs B1 :|: S) (add_fundefs B1 fm) (def_funs B1 B1 rho1 rho1) (def_funs B2 B2 rho2 rho2) i
+                (set_list (combine (all_fun_name B1) (all_fun_name B2)) sig).
+  Proof.
+    revert S fm rho1 rho2 i sig B1 B2. induction k as [k IHk] using lt_wf_rec1.
+    intros S fm rho1 rho2 i sig B1 B2 Hf Hrel Hun Hsub Hdis Hdis'.
+    intros f ft xs e rhoc B' f' HSin Heq1 Heq2.
+    destruct (Decidable_name_in_fundefs B1) as [Dec]. destruct (Dec f).
+    - rewrite def_funs_eq in Heq2; eauto. inv Heq2.
+      edestruct name_in_fundefs_find_def_is_Some. eassumption. destructAll.
+      erewrite add_fundefs_in in Heq1; [| eassumption ]. inv Heq1. split; eauto.
+      split; eauto. split.
+      + eapply preord_env_P_inj_antimon. eassumption. eapply Setminus_Included_Included_Union.
+        eapply Included_trans. eapply occurs_free_in_fun. eapply find_def_correct. eassumption. sets.
+      + destruct k; eauto. rewrite <- fun_map_inv_eq. eapply fun_map_inv_antimon. eapply IHk.
+        omega. eapply fun_map_inv_mon. eassumption. omega. eassumption. eassumption.
+        eassumption. now sets. now sets. eapply Setminus_Included_Included_Union. 
+        eapply Included_trans. eapply occurs_free_in_fun. eapply find_def_correct. eassumption.
+        sets.
+    - rewrite def_funs_neq in Heq2; eauto.
+      rewrite add_fundefs_not_in in Heq1; [| eassumption ]. inv HSin. contradiction.
+      edestruct Hf. eassumption. eassumption. eassumption. destructAll. split; eauto. split; eauto. split.
+      + eapply preord_env_P_inj_def_funs_neq_r.
+        rewrite apply_r_set_list_f_eq. eapply preord_env_P_inj_extend_lst_not_In_P_r.
+        eassumption.
+        * rewrite <- Same_set_all_fun_name.
+          eapply Disjoint_Included; [| | eapply Hdis ]. eapply Included_Union_preserv_r.
+          eapply occurs_free_fun_map_get. eassumption. reflexivity. 
+        * rewrite apply_r_set_list_f_eq. eapply Disjoint_Included_l. 
+          intros x Hc. destruct Hc. destructAll.
+          rewrite extend_lst_gso. eapply In_image. eassumption.
+          rewrite <- Same_set_all_fun_name. intros Hc. eapply Hdis. constructor.
+          eassumption. right.
+          eapply occurs_free_fun_map_get. eassumption. eassumption.
+          eapply Disjoint_sym. eapply Disjoint_Included_r; [| eassumption ]. apply image_monotonic.
+          eapply occurs_free_fun_map_get. eassumption.
+      + destruct k; eauto. rewrite <- fun_map_inv_eq in *.
+        eapply fun_map_inv_add_fundefs. eapply fun_map_inv_def_funs_Disjoint; try eassumption.
+        * eapply Union_Disjoint_r; [| sets ].
+          eapply Disjoint_Included_r; [| eassumption ]. eapply Included_Union_preserv_r.
+          eapply occurs_free_fun_map_get. eassumption.
+        * eapply Union_Disjoint_r; [| sets ].
+          eapply Disjoint_Included_r; [| eassumption ]. eapply Included_Union_preserv_r.
+          eapply occurs_free_fun_map_get. eassumption.          
+  Qed.
+
+  Lemma fun_map_inv_def_funs k S fm rho1 rho2 i sig B1 B2 :
+    fun_map_inv k S fm rho1 rho2 i sig ->
+        
+    Disjoint _ (name_in_fundefs B1) (S :|: occurs_free_fun_map fm) ->
+    Disjoint _ (name_in_fundefs B2) (image (apply_r sig) (occurs_free_fun_map fm)) ->        
+    Disjoint _ (name_in_fundefs B1) (Dom_map fm) ->
+    
+    fun_map_inv k (name_in_fundefs B1 :|: S) fm (def_funs B1 B1 rho1 rho1) (def_funs B2 B2 rho2 rho2) i
+                (set_list (combine (all_fun_name B1) (all_fun_name B2)) sig).
+  Proof.
+    revert S fm rho1 rho2 i sig B1 B2. induction k as [k IHk] using lt_wf_rec1.
+    intros S fm rho1 rho2 i sig B1 B2 Hf (* Hrel *) (* Hun Hsub *) Hdis Hdis' Hdis''.
+    intros f ft xs e rhoc B' f' HSin Heq1 Heq2.
+    destruct (Decidable_name_in_fundefs B1) as [Dec]. destruct (Dec f).
+    - exfalso.
+      eapply Hdis''. constructor. eassumption. eexists; eauto.
+    - rewrite def_funs_neq in Heq2; eauto. inv HSin. contradiction.
+      edestruct Hf. eassumption. eassumption. eassumption. destructAll. split; eauto. split; eauto. split.
+      + eapply preord_env_P_inj_def_funs_neq_r.
+        rewrite apply_r_set_list_f_eq. eapply preord_env_P_inj_extend_lst_not_In_P_r.
+        eassumption.
+        * rewrite <- Same_set_all_fun_name.
+          eapply Disjoint_Included; [| | eapply Hdis ]. eapply Included_Union_preserv_r.
+          eapply occurs_free_fun_map_get. eassumption. reflexivity. 
+        * rewrite apply_r_set_list_f_eq. eapply Disjoint_Included_l. 
+          intros x Hc. destruct Hc. destructAll.
+          rewrite extend_lst_gso. eapply In_image. eassumption.
+          rewrite <- Same_set_all_fun_name. intros Hc. eapply Hdis. constructor.
+          eassumption. right.
+          eapply occurs_free_fun_map_get. eassumption. eassumption.
+          eapply Disjoint_sym. eapply Disjoint_Included_r; [| eassumption ]. apply image_monotonic.
+          eapply occurs_free_fun_map_get. eassumption.
+      + destruct k; eauto. rewrite <- fun_map_inv_eq in *.
+        eapply fun_map_inv_def_funs_Disjoint; try eassumption.
+        * eapply Union_Disjoint_r; [| clear Hdis' Hdis''; sets ].
+          eapply Disjoint_Included_r; [| eapply Hdis ]. eapply Included_Union_preserv_r.
+          eapply occurs_free_fun_map_get. eassumption.
+  Qed.
+
+  Lemma fun_map_inv_i_mon k S fm rho1 rho2 i i' sig :
+    fun_map_inv k S fm rho1 rho2 i sig ->
+    (i' <= i)%nat ->
+    fun_map_inv k S fm rho1 rho2 i' sig.
+  Proof.
+    revert k S fm rho1 rho2 i i' sig. induction k as [k' IHk] using lt_wf_rec1; intros.
+    intros. intro; intros. edestruct H; eauto. destructAll. split; eauto. split; eauto. split; eauto.
+    eapply preord_env_P_inj_monotonic; eassumption.
+    destruct k'; eauto. rewrite <- fun_map_inv_eq in *. eapply IHk; eauto.
+  Qed.
+
+  Lemma fun_map_inv_remove k S fm rho1 rho2 i sig f:
+    fun_map_inv k S fm rho1 rho2 i sig ->
+    fun_map_inv k S (M.remove f fm) rho1 rho2 i sig.
+  Proof.
+    revert k S fm rho1 rho2 i sig f. induction k as [k' IHk] using lt_wf_rec1; intros.
+    intros. intro; intros.
+    destruct (peq f f0). subst. rewrite M.grs in H1. inv H1. rewrite M.gro in H1; eauto.
+    edestruct H; eauto. destructAll. split; eauto. split; eauto. split; eauto.
+    destruct k'; eauto. rewrite <- fun_map_inv_eq in *. eapply IHk; eauto.
+  Qed.
+
+  
+
+  (* [fun_map_vars] *)
+  
+  Definition fun_map_vars (fm : fun_map) (F : Ensemble var) (sig : subst) :=
+    forall f ft xs e,
+      fm ! f = Some (ft, xs, e) ->
+      unique_bindings e /\
+      NoDup xs /\
+      Disjoint _ (bound_var e) (FromList xs :|: occurs_free e) /\
+      Disjoint _ (bound_var e) (Dom_map fm) /\
+      Disjoint _ (bound_var e :|: FromList xs) (occurs_free_fun_map (M.remove f fm)) /\
+      Disjoint _ (bound_var e :|: occurs_free e) (bound_var_fun_map (M.remove f fm)) /\      
+      Disjoint _ (FromList xs) (Dom_map fm) /\      
+      Disjoint _ F (bound_var e :|: image (apply_r sig) (occurs_free e \\ FromList xs)).
+
+  Lemma fun_map_vars_antimon fm F F' sig :
+    fun_map_vars fm F sig ->
+    F' \subset F ->
+    fun_map_vars fm F' sig.
+  Proof.
+    intros Hfm Hsub; intro; intros. eapply Hfm in H. destructAll.
+    do 6 (split; eauto). sets.
+  Qed.
+
+  Instance fm_map_vars_Proper fm : Proper (Same_set _ ==> eq ==> iff) (fun_map_vars fm).
+  Proof.
+    repeat (intro; intros). subst. split; intros.
+    intro; intros. eapply H0 in H1. rewrite H in H1. eauto.
+    intro; intros. eapply H0 in H1. rewrite <- H in H1. eauto.
+  Qed.
+
+
+  Lemma fun_map_vars_set fm F sig x v :
+    fun_map_vars fm F sig ->
+    fun_map_vars fm (F \\ [set v]) (M.set x v sig).
+  Proof.
+    intros Hfm; intro; intros. eapply Hfm in H. destructAll.
+    do 8 (split; eauto). eapply Union_Disjoint_r. now sets.
+    eapply Disjoint_Included_r. eapply image_apply_r_set.
+    eapply Union_Disjoint_r. now sets. now xsets.
+  Qed.
+  
+  Lemma fun_map_vars_set_list fm F sig xs vs :
+    fun_map_vars fm F sig ->
+    fun_map_vars fm (F \\ FromList vs) (set_list (combine xs vs) sig).
+  Proof.
+    revert F vs sig. induction xs; intros F vs sig.
+    - simpl. intros Hin. eapply fun_map_vars_antimon. eassumption.
+      now sets.
+    - destruct vs; simpl.
+      + intros Hf. eapply fun_map_vars_antimon. eassumption. sets.
+      + intros Hfm. simpl. repeat normalize_sets. rewrite Union_commut.
+        rewrite <- Setminus_Union. eapply fun_map_vars_set. 
+        simpl. eapply IHxs; eauto.
+  Qed.
+
+ 
   Lemma fun_map_vars_def_funs fm S sig B xs :
     fun_map_vars fm S sig ->
     unique_bindings_fundefs B ->
 
     Disjoint _ (bound_var_fundefs B) (occurs_free_fundefs B :|: occurs_free_fun_map fm) ->
-    Disjoint _ (occurs_free_fundefs B :|: bound_var_fundefs B) (bound_var_fun_map' fm) ->
+    Disjoint _ (occurs_free_fundefs B :|: bound_var_fundefs B) (bound_var_fun_map fm) ->
     
-    Disjoint _ (bound_var_fundefs B \\ funname_in_fundefs B \\ name_in_fundefs B) (Dom_map fm :|: funname_fun_map fm) ->
+    Disjoint _ (bound_var_fundefs B) (Dom_map fm) ->
     Disjoint _ (S \\ FromList xs) (bound_var_fundefs B :|: image (apply_r sig) (occurs_free_fundefs B)) ->    
-    Disjoint _ (name_in_fundefs B) (bound_var_fun_map fm) ->
-    Disjoint _ (funname_in_fundefs B) (bound_var_fun_map fm) ->
     
     Datatypes.length (all_fun_name B) = Datatypes.length xs ->
     
     fun_map_vars (add_fundefs B fm) (S \\ FromList xs) (set_list (combine (all_fun_name B) xs) sig).
   Proof.
-    intros Hfm Hun Hdis1 Hdis' Hdis2 Hdis3 Hdis4 Hdis5 Hlen x ft ys e Hget. destruct (Decidable_name_in_fundefs B). destruct (Dec x).
+    intros Hfm Hun Hdis1 Hdis' Hdis2 Hdis3 (* Hdis4 Hdis5 *) Hlen x ft ys e Hget. destruct (Decidable_name_in_fundefs B). destruct (Dec x).
     - edestruct name_in_fundefs_find_def_is_Some; eauto. destructAll. erewrite add_fundefs_in in Hget; eauto.
       inv Hget. edestruct unique_bindings_fun_in_fundefs. eapply find_def_correct. eassumption. eassumption. destructAll.
       assert (Hin1 : bound_var e \subset bound_var_fundefs B).
@@ -1136,43 +881,34 @@ Section Inline_correct.
       split. now eauto. split. now eauto. split; [| split; [| split; [| split; [| split; [| split ]]]]].
       + eapply Union_Disjoint_r. now sets.
         eapply fun_in_fundefs_Disjoint_bound_Var_occurs_free. eapply find_def_correct. eassumption.
-        eassumption. now sets.        
-      + rewrite Dom_map_add_fundefs. eapply Union_Disjoint_r. eapply Union_Disjoint_r. now sets.
-        * eapply Disjoint_Included; [| | eapply Hdis2 ]. now sets.
-          eapply Included_Setminus. now sets. 
-          eapply fun_in_fundefs_bound_var_Setminus. eapply find_def_correct. eassumption. eassumption.
-        * eapply Disjoint_Included_r. eapply funname_fun_map_add_fundefs. eapply Union_Disjoint_r.
-          ++ eapply Disjoint_Included_l. eapply fun_in_fundefs_bound_var_Setminus. eapply find_def_correct. eassumption.
-             eassumption. now sets.
-          ++ eapply Disjoint_Included_l. eapply fun_in_fundefs_bound_var_Setminus'. eapply find_def_correct. eassumption.
-             eassumption. now sets.
+        eassumption. clear Hdis2. sets.
+      + rewrite Dom_map_add_fundefs. eapply Union_Disjoint_r. now sets.
+        eapply Disjoint_Included; [| | eapply Hdis2 ]. now sets.
+        eapply Included_trans; [| eapply fun_in_fundefs_bound_var_fundefs; eapply find_def_correct; eauto ]. now sets.
       + eapply Disjoint_Included_r. eapply occurs_free_fun_map_remove_add_fundefs. eapply Union_Disjoint_r; [ eapply Union_Disjoint_r | ].
-        * eapply Disjoint_Included_l. eapply Union_Included. eassumption. eassumption. sets.
+        * eapply Disjoint_Included_l. eapply Union_Included. eassumption.
+          eapply Included_trans; [| eapply fun_in_fundefs_bound_var_fundefs; eapply find_def_correct; eauto ]. now sets.
+          clear Hdis2. sets.
         * sets.
         * eapply Disjoint_Included_r. eapply occurs_free_fun_map_remove.
-          eapply Disjoint_Included_l. eapply Union_Included; eassumption. sets.
+          eapply Disjoint_Included_l. eapply Union_Included; eassumption. clear Hdis2. sets.
       + eapply Disjoint_Included_l.
         * eapply Included_Union_compat. reflexivity. eapply occurs_free_in_fun. eapply find_def_correct. eassumption.
         * rewrite Union_assoc. eapply Union_Disjoint_l.
           -- eapply Disjoint_Included_r.
-             eapply bound_var_fun_map_remove_add_fundefs_un''. eassumption. eassumption. eapply Union_Disjoint_r.
+             eapply bound_var_fun_map_remove_add_fundefs_un. eassumption. eassumption. eapply Union_Disjoint_r.
              ++ sets.
              ++ eapply Disjoint_Included. eapply bound_var_fun_map_remove.
                 eapply Union_Included; eassumption. sets.
           -- eapply Disjoint_Included_r. eapply bound_var_fun_map_remove_add_fundefs_un'. eassumption.
              eapply Union_Disjoint_r.
-             ++ sets.
+             ++ eapply Union_Disjoint_l. now sets. clear Hdis2. sets.
              ++ eapply Disjoint_Included_r. eapply bound_var_fun_map_remove.
                 eapply Union_Disjoint_l; [| now sets ]. eapply Disjoint_Included_l.
                 eapply name_in_fundefs_bound_var_fundefs. sets.
       + rewrite Dom_map_add_fundefs. eapply Union_Disjoint_r. eassumption.
         eapply Disjoint_Included_l.
-        eapply Included_Setminus. eassumption. 
-        eapply fun_in_fundefs_FromList_subset. eapply find_def_correct. eassumption. eassumption.
-        now sets.
-      + eapply Disjoint_Included_r. eapply bound_var_fun_map_add_fundefs_un. eassumption.
-        eapply Disjoint_Included_l. eapply fun_in_fundefs_funname_in_exp. eapply find_def_correct. eassumption.
-        eapply Union_Disjoint_r. now sets. eassumption.
+        eapply Included_Setminus. eassumption. eassumption. sets.
       + eapply Union_Disjoint_r. now sets. eapply Disjoint_Included_r.
         eapply image_apply_r_set_list. now eauto. eapply Union_Disjoint_r. now sets.
         rewrite <- Same_set_all_fun_name.
@@ -1182,42 +918,52 @@ Section Inline_correct.
     - rewrite add_fundefs_not_in in Hget; eauto. edestruct Hfm. eassumption. destructAll.
       split; eauto. split; eauto. split; [| split; [| split; [| split; [| split; [| split ]]]]].
       + now sets.
-      + rewrite Dom_map_add_fundefs. eapply Union_Disjoint_r. eapply Union_Disjoint_r. 
-        * eapply Disjoint_sym. eapply Disjoint_Included_r; [| eassumption ].
+      + rewrite Dom_map_add_fundefs. eapply Union_Disjoint_r.
+        * eapply Disjoint_sym. eapply Disjoint_Included; [| | eapply Hdis' ].
           eapply Included_trans; [| eapply bound_var_fun_map_get; eauto ]. now sets.
+          eapply Included_trans. eapply name_in_fundefs_bound_var_fundefs. sets.
         * sets.
-        * eapply Disjoint_Included_r. eapply funname_fun_map_add_fundefs. eapply Union_Disjoint_r; [| now sets ].
-          eapply Disjoint_sym. eapply Disjoint_Included_r; [| eassumption ]. 
-          eapply Included_trans; [| eapply bound_var_fun_map_get; eauto ]. sets.
       + eapply Disjoint_Included_r. eapply occurs_free_fun_map_remove_add_fundefs.
         eapply Union_Disjoint_r; [| now sets ].
         eapply Disjoint_Included_l.
-        now eapply bound_var_fun_map_get'; eauto.
+        now eapply bound_var_fun_map_get; eauto.
         eapply Disjoint_sym. eapply Disjoint_Included_l; [| eassumption ]. eapply Included_Union_compat.
         reflexivity. eapply name_in_fundefs_bound_var_fundefs. 
       + eapply Disjoint_Included_r. eapply bound_var_fun_map_remove_add_fundefs_un'.
         eassumption. eapply Union_Disjoint_r; [| now sets ]. eapply Union_Disjoint_l.
         * eapply Disjoint_sym. eapply Disjoint_Included; [| | eapply Hdis' ].
-          eapply Included_trans; [| eapply bound_var_fun_map_get'; eauto ]. sets. sets.
+          eapply Included_trans; [| eapply bound_var_fun_map_get; eauto ]. sets. sets.
         * eapply Disjoint_Included_l. eapply Included_Union_Setminus with (s2 := FromList ys). tci.
           eapply Union_Disjoint_l. 
           -- eapply Disjoint_sym. eapply Disjoint_Included; [| | eapply Hdis1 ].
              eapply Included_Union_preserv_r. eapply Included_trans; [| eapply occurs_free_fun_map_get; eauto ]. sets.
              sets.
           -- eapply Disjoint_sym. eapply Disjoint_Included; [| | eapply Hdis' ].
-             eapply Included_trans; [| eapply bound_var_fun_map_get'; eauto ]. sets. sets.
-      + rewrite Dom_map_add_fundefs. eapply Union_Disjoint_r; [| now sets ].
-        eapply Disjoint_sym. eapply Disjoint_Included_r; [| eassumption ].
-        eapply Included_trans; [| eapply bound_var_fun_map_get; eauto ]. now sets.
-      + eapply Disjoint_Included_r. eapply bound_var_fun_map_add_fundefs_un. eassumption.
-        eapply Union_Disjoint_r; [| eassumption ].
-        * eapply Disjoint_sym. eapply Disjoint_Included_r. eapply funname_fun_map_fun_map_get. eassumption.
-          sets.
+             eapply Included_trans; [| eapply bound_var_fun_map_get; eauto ]. sets. sets.
+      + rewrite Dom_map_add_fundefs. eapply Union_Disjoint_r.
+        eapply Disjoint_sym. eapply Disjoint_Included; [| | eapply Hdis' ].
+        eapply Included_trans; [| eapply bound_var_fun_map_get; eauto ]. sets.
+        eapply Included_trans. eapply name_in_fundefs_bound_var_fundefs. sets.
+        sets.
       + eapply Union_Disjoint_r. now sets. 
         eapply Disjoint_Included_r. eapply image_apply_r_set_list. eassumption.
         eapply Union_Disjoint_r. now sets. xsets.
   Qed.
-  
+
+  Lemma fun_map_vars_inv_remove S fm sig f :
+    fun_map_vars fm S sig ->
+    fun_map_vars (M.remove f fm) S sig.
+  Proof.
+    intros Hfm. intro; intros.
+    destruct (peq f f0). subst. rewrite M.grs in H. inv H. rewrite M.gro in H; eauto.
+    edestruct Hfm. eassumption. destructAll. repeat (split; [ now eauto |]).
+    split; [| split; [| split; [| split ]]]; eauto.
+    - rewrite Dom_map_remove. sets.
+    - sets. eapply Disjoint_Included_r. eapply occurs_free_fun_map_remove'. sets.
+    - sets. eapply Disjoint_Included_r. eapply bound_var_fun_map_remove'. sets.
+    - rewrite Dom_map_remove. sets.
+  Qed.
+
   Opaque preord_exp'.
 
 
@@ -1246,52 +992,15 @@ Section Inline_correct.
     | _ => True
     end.
              
-  Lemma fun_map_inv_i_mon k S fm rho1 rho2 i i' sig :
-    fun_map_inv k S fm rho1 rho2 i sig ->
-    (i' <= i)%nat ->
-    fun_map_inv k S fm rho1 rho2 i' sig.
-  Proof.
-    revert k S fm rho1 rho2 i i' sig. induction k as [k' IHk] using lt_wf_rec1; intros.
-    intros. intro; intros. edestruct H; eauto. destructAll. split; eauto. split; eauto. split; eauto.
-    eapply preord_env_P_inj_monotonic; eassumption.
-    destruct k'; eauto. rewrite <- fun_map_inv_eq in *. eapply IHk; eauto.
-  Qed.
-
-  Lemma fun_map_inv_remove k S fm rho1 rho2 i sig f:
-    fun_map_inv k S fm rho1 rho2 i sig ->
-    fun_map_inv k S (M.remove f fm) rho1 rho2 i sig.
-  Proof.
-    revert k S fm rho1 rho2 i sig f. induction k as [k' IHk] using lt_wf_rec1; intros.
-    intros. intro; intros.
-    destruct (peq f f0). subst. rewrite M.grs in H1. inv H1. rewrite M.gro in H1; eauto.
-    edestruct H; eauto. destructAll. split; eauto. split; eauto. split; eauto.
-    destruct k'; eauto. rewrite <- fun_map_inv_eq in *. eapply IHk; eauto.
-  Qed.
-
-  Lemma fun_map_vars_inv_remove S fm sig f :
-    fun_map_vars fm S sig ->
-    fun_map_vars (M.remove f fm) S sig.
-  Proof.
-    intros Hfm. intro; intros.
-    destruct (peq f f0). subst. rewrite M.grs in H. inv H. rewrite M.gro in H; eauto.
-    edestruct Hfm. eassumption. destructAll. repeat (split; [ now eauto |]).
-    split; [| split; [| split; [| split; [| split ]]]]; eauto.
-    admit.
-    admit.
-    admit.
-    rewrite Dom_map_remove. sets.
-    admit.
-  Admitted.
-  
+   
   Lemma inline_correct_mut d : 
     (forall e sig fm st S
             (Hun : unique_bindings e)
             (Hdis1 : Disjoint _ (bound_var e) (occurs_free e :|: occurs_free_fun_map fm))
-            (Hdis1' : Disjoint _ (bound_var e :|: bound_var_fun_map' fm) (image (apply_r sig) (occurs_free e :|: occurs_free_fun_map fm)))
-            (Hdis2 : Disjoint _ S ((bound_var e :|: bound_var_fun_map' fm) :|: image (apply_r sig) (occurs_free e :|: occurs_free_fun_map fm)))
-            (Hdis3 : Disjoint _ (bound_var e \\ funname_in_exp e) (Dom_map fm :|: funname_fun_map fm))
-            (Hdis4 : Disjoint _ (funname_in_exp e) (bound_var_fun_map fm))
-            (Hdis5 : Disjoint _ (bound_var_fun_map' fm) (bound_var e :|: occurs_free e))
+            (Hdis1' : Disjoint _ (bound_var e :|: bound_var_fun_map fm) (image (apply_r sig) (occurs_free e :|: occurs_free_fun_map fm)))
+            (Hdis2 : Disjoint _ S ((bound_var e :|: bound_var_fun_map fm) :|: image (apply_r sig) (occurs_free e :|: occurs_free_fun_map fm)))
+            (Hdis3 : Disjoint _ (bound_var e) (Dom_map fm))
+            (Hdis5 : Disjoint _ (bound_var_fun_map fm) (bound_var e :|: occurs_free e))
             
             (Hfm : fun_map_vars fm S sig),
         {{ fun _ s => fresh S (next_var (fst s)) }}
@@ -1308,17 +1017,15 @@ Section Inline_correct.
 
     (forall B sig sig0 fm st S
             (Hun : unique_bindings_fundefs B)
-            (Hdis1 : Disjoint _ (bound_var_fundefs B (* :|: bound_var_fun_map' fm *)) (occurs_free_fundefs B :|: (occurs_free_fun_map fm \\ name_in_fundefs B)))
-            (Hdis1' : Disjoint _ (bound_var_fundefs B :|: bound_var_fun_map' fm) (image (apply_r sig) (occurs_free_fundefs B :|: occurs_free_fun_map fm)))
-
-            (Hdis2 : Disjoint _ S ((bound_var_fundefs B :|: bound_var_fun_map' fm):|: image (apply_r sig) (occurs_free_fundefs B :|: occurs_free_fun_map fm)))
-            (Hdis3 : Disjoint _ (bound_var_fundefs B \\ name_in_fundefs B \\ funname_in_fundefs B) (Dom_map fm :|: funname_fun_map fm))
-            (Hdis4 : Disjoint _ (funname_in_fundefs B) (bound_var_fun_map fm))
-            (Hdis5 : Disjoint _ (bound_var_fun_map' fm) (bound_var_fundefs B :|: occurs_free_fundefs B))
+            (Hdis1 : Disjoint _ (bound_var_fundefs B) (occurs_free_fundefs B :|: (occurs_free_fun_map fm \\ name_in_fundefs B)))
+            (Hdis1' : Disjoint _ (bound_var_fundefs B :|: bound_var_fun_map fm) (image (apply_r sig) (occurs_free_fundefs B :|: occurs_free_fun_map fm)))
+            (Hdis2 : Disjoint _ S ((bound_var_fundefs B :|: bound_var_fun_map fm):|: image (apply_r sig) (occurs_free_fundefs B :|: occurs_free_fun_map fm)))
+            (Hdis3 : Disjoint _ (bound_var_fundefs B) (Dom_map fm))
+            (Hdis5 : Disjoint _ (bound_var_fun_map fm) (bound_var_fundefs B :|: occurs_free_fundefs B))
                         
             (Hfm : fun_map_vars fm S sig)
             (Hnames1 : NoDup (apply_r_list sig (all_fun_name B)))
-            (Hnames2 : Disjoint _ (S :|: (bound_var_fundefs B :|: bound_var_fun_map' fm)) (FromList (apply_r_list sig (all_fun_name B)))), 
+            (Hnames2 : Disjoint _ (S :|: (bound_var_fundefs B :|: bound_var_fun_map fm)) (FromList (apply_r_list sig (all_fun_name B)))), 
         {{ fun _ s => fresh S (next_var (fst s)) }}
           beta_contract_fundefs St IH d sig0 sig fm B st
         {{ fun _ s B' s' =>
@@ -1364,7 +1071,6 @@ Section Inline_correct.
         eapply Disjoint_Included; [| | eapply Hdis2 ].
         rewrite Setminus_Union_distr. rewrite !image_Union. now xsets. now sets.
       + eapply Disjoint_Included_l; [| eassumption ]. normalize_bound_var. sets.
-      + eassumption.
       + eapply Disjoint_Included_r. eapply bound_var_occurs_free_Econstr_Included. eassumption.
       + eapply fun_map_vars_set. eassumption.
       + intros e' w2. eapply return_triple.
@@ -1400,9 +1106,7 @@ Section Inline_correct.
           -- eapply fun_map_inv_antimon. eapply fun_map_inv_set. eapply fun_map_inv_i_mon. eassumption. omega.
              intros Hc. inv Hc.
              ++ eapply Hdis1. normalize_bound_var. normalize_occurs_free. constructor. now right. eauto.
-             ++ eapply Hdis3. constructor. normalize_bound_var. simpl. constructor. now right.
-                intros Hc. eapply H1. eapply funname_in_exp_subset. eassumption.
-                now left; eauto.
+             ++ eapply Hdis3. constructor. normalize_bound_var. now right. eassumption.
              ++ intros Hc. eapply Hdis2. constructor; try eassumption. rewrite image_Union. do 2 right. eassumption.
              ++ normalize_occurs_free. rewrite !Union_assoc. rewrite Union_Setminus_Included; sets; tci.
     - (* Ecase [] *)
@@ -1426,12 +1130,12 @@ Section Inline_correct.
           eapply Disjoint_Included; [| | eapply Hdis1' ]; sets.
         * repeat normalize_bound_var_in_ctx. repeat normalize_occurs_free_in_ctx.
           xsets.
-        * repeat normalize_bound_var_in_ctx. repeat normalize_occurs_free_in_ctx.
-          eapply Disjoint_Included_l; [| eassumption ]. simpl. rewrite Setminus_Union_distr.
-          eapply Included_Union_preserv_l. rewrite <- Setminus_Union. eapply Included_Setminus; [| sets ].          
-          eapply Disjoint_Included; [| | eapply H5 ].
-          eapply Included_trans; [| eapply funname_in_exp_subset ]. now sets. now sets.
-        * sets.
+        * repeat normalize_bound_var_in_ctx. repeat normalize_occurs_free_in_ctx. now sets.
+          (* eapply Disjoint_Included_l; [| eassumption ]. simpl. now sets. rewrite Setminus_Union_distr. *)
+          (* eapply Included_Union_preserv_l. rewrite <- Setminus_Union. eapply Included_Setminus; [| sets ].           *)
+          (* eapply Disjoint_Included; [| | eapply H5 ]. *)
+          (* eapply Included_trans; [| eapply funname_in_exp_subset ]. now sets. now sets. *)
+        (* * sets. *)
         * eapply Disjoint_Included_r. eapply bound_var_occurs_free_Ecase_Included. 2:{ eassumption. }
           now left.
         * eassumption.
@@ -1452,13 +1156,7 @@ Section Inline_correct.
              eapply Disjoint_Included; [| | eapply Hdis1' ]; sets.
           -- repeat normalize_bound_var_in_ctx. repeat normalize_occurs_free_in_ctx.
              xsets.
-          -- repeat normalize_bound_var_in_ctx. repeat normalize_occurs_free_in_ctx.
-             eapply Disjoint_Included_l; [| eassumption ]. simpl. rewrite Setminus_Union_distr.
-             eapply Included_Union_preserv_r. rewrite Union_commut. rewrite <- Setminus_Union.
-             eapply Included_Setminus; [| now sets ].             
-             eapply Disjoint_sym. eapply Disjoint_Included; [| | eapply H5 ]. now sets.
-             eapply funname_in_exp_subset.
-          -- sets.
+          -- repeat normalize_bound_var_in_ctx. repeat normalize_occurs_free_in_ctx. now sets.
           -- eapply Disjoint_Included_r. eapply bound_var_occurs_free_Ecase_cons_Included. eassumption.
           -- eassumption.
         * intros ce w'. simpl. eapply pre_curry_l. intros Hbv. eapply pre_curry_l. intros Hleq.
@@ -1517,7 +1215,6 @@ Section Inline_correct.
         eapply Disjoint_Included; [| | eapply Hdis2 ].
         rewrite Setminus_Union_distr. rewrite !image_Union. now xsets. now sets.
       + eapply Disjoint_Included_l; [| eassumption ]. normalize_bound_var. sets.
-      + eassumption.
       + eapply Disjoint_Included_r. eapply bound_var_occurs_free_Eproj_Included. eassumption.
       + eapply fun_map_vars_set. eassumption.
       + intros e' w2. eapply return_triple.
@@ -1550,9 +1247,7 @@ Section Inline_correct.
           -- eapply fun_map_inv_antimon. eapply fun_map_inv_set. eapply fun_map_inv_i_mon. eassumption. omega.
              intros Hc. inv Hc. 
              ++ eapply Hdis1. normalize_bound_var. constructor. now right. now right; eauto.
-             ++ eapply Hdis3. constructor. normalize_bound_var. simpl. constructor. now right.
-                intros Hc. eapply H1. eapply funname_in_exp_subset. eassumption.
-                now left; eauto.
+             ++ eapply Hdis3. constructor. normalize_bound_var. now right. eassumption. 
              ++ intros Hc. eapply Hdis2. constructor; try eassumption. rewrite image_Union. do 2 right. eassumption.
              ++ normalize_occurs_free. rewrite !Union_assoc. rewrite Union_Setminus_Included; sets; tci.
     - (* Eletapp *)
@@ -1581,7 +1276,6 @@ Section Inline_correct.
           eapply Disjoint_Included; [| | eapply Hdis2 ]; [| now sets ].
           eapply Included_Union_preserv_r. eapply image_monotonic. rewrite Setminus_Union_distr. sets. 
         - eapply Disjoint_Included_l; [| eassumption ]. normalize_bound_var. sets.
-        - eassumption.
         - eapply Disjoint_Included_r. eapply bound_var_occurs_free_Eletapp_Included. eassumption.
         - eapply fun_map_vars_set. eassumption.
         - intros e' w2. eapply return_triple.
@@ -1618,9 +1312,7 @@ Section Inline_correct.
             -- eapply fun_map_inv_antimon. eapply fun_map_inv_set. eapply fun_map_inv_i_mon. eassumption. omega.
                intros Hc. inv Hc.
                ++ eapply Hdis1. constructor. normalize_bound_var. now right. right; eassumption.
-               ++ eapply Hdis3. constructor. normalize_bound_var. simpl. constructor. now right.
-                  intros Hc. eapply H1. eapply funname_in_exp_subset. eassumption.
-                  now left; eauto.
+               ++ eapply Hdis3. constructor. normalize_bound_var. now right. eassumption. 
                ++ intros Hc. eapply Hdis2. constructor. eassumption. rewrite image_Union.
                   do 2 right. eassumption.
                ++ normalize_occurs_free. rewrite !Union_assoc. rewrite Union_Setminus_Included; sets; tci. }        
@@ -1635,14 +1327,14 @@ Section Inline_correct.
             - do 2 eapply frame_rule. eapply pre_transfer_r. eapply IHd.
               + omega.
               + eassumption.
-              + sets.
+              + eapply Union_Disjoint_r. clear H3. now sets. now sets.
               + eapply Disjoint_Included_r. eapply image_apply_r_set_list. unfold apply_r_list. rewrite map_length. eassumption.
                 eapply Union_Disjoint_r.
                 * eapply Disjoint_Included; [ | | eapply Hdis1' ].
                   rewrite FromList_apply_list. normalize_occurs_free. rewrite !image_Union. now sets.
                   eapply Union_Included.
                   -- eapply Included_Union_preserv_r. 
-                     eapply Included_trans; [| eapply bound_var_fun_map_get'; eauto ]. sets.
+                     eapply Included_trans; [| eapply bound_var_fun_map_get; eauto ]. sets.
                   -- eapply Included_trans. eapply bound_var_fun_map_remove. sets. 
                 * eapply Disjoint_Included; [| | eapply Hdis1' ]. rewrite image_Union.
                   eapply Included_Union_preserv_r. eapply image_monotonic. rewrite Setminus_Union_distr. 
@@ -1652,9 +1344,9 @@ Section Inline_correct.
                      sets.
                   -- eapply Union_Included; [|  eapply Included_trans; [ eapply bound_var_fun_map_remove |]; sets ].
                      eapply Included_Union_preserv_r.
-                     eapply Included_trans; [| eapply bound_var_fun_map_get'; eauto ]. now sets.
+                     eapply Included_trans; [| eapply bound_var_fun_map_get; eauto ]. now sets.
               + repeat normalize_bound_var_in_ctx. repeat normalize_occurs_free_in_ctx. eapply Union_Disjoint_r.
-                eapply Union_Disjoint_r. now sets. clear H9.
+                eapply Union_Disjoint_r. now sets. clear H8.
                 eapply Disjoint_Included_r. eapply bound_var_fun_map_remove. now sets.
                 eapply Disjoint_Included_r.
                 eapply image_apply_r_set_list. unfold apply_r_list. rewrite map_length. eassumption. 
@@ -1663,16 +1355,13 @@ Section Inline_correct.
                 eapply Disjoint_Included; [| | eapply Hdis2 ]; [| now sets ]. rewrite !image_Union. now sets.
                 
                 rewrite !Setminus_Union_distr. rewrite image_Union. eapply Union_Disjoint_r.
-                eapply Disjoint_Included; [| | eapply H9 ]; now sets.
+                eapply Disjoint_Included; [| | eapply H8 ]; now sets.
                 eapply Disjoint_Included; [| | eapply Hdis2 ].
                 eapply Included_trans. eapply image_monotonic. eapply Included_Setminus_compat.
                 eapply occurs_free_fun_map_remove. reflexivity. now sets. now sets.                
-              + eapply Disjoint_Included_r; [| eassumption ]. eapply Included_Union_compat.
-                rewrite Dom_map_remove. sets. admit. (* easy *) 
-              + admit. (* easy *) 
+              + rewrite Dom_map_remove. sets.
               + sets.
               + eapply fun_map_vars_inv_remove.
-                (* Make lemma if needed about fun_map_vars fm S (set_list (combine xs (apply_r_list sig l)) sig) *)
                 intros ? ? ? ? ?.
                 edestruct Hfm; eauto. destructAll.
                 repeat (split; [ now eauto |]). eapply Union_Disjoint_r. now sets.
@@ -1687,25 +1376,25 @@ Section Inline_correct.
               eapply pre_strenghtening.
               { intros. destructAll.
                 assert (Hfr' : fresh (S \\ [set z] \\ bound_var ei) (next_var (fst s0))).
-                { intros u Hleq'. constructor. eapply H10; eauto.
-                  intros Hnin. eapply H14 in Hnin. unfold Ensembles.In, Range in Hnin. zify. omega. }
+                { intros u Hleq'. constructor. eapply H9; eauto.
+                  intros Hnin. eapply H13 in Hnin. unfold Ensembles.In, Range in Hnin. zify. omega. }
                 assert (Hbv : bound_var ei \subset S \\ [set z]).
                 { eapply Included_trans. eassumption. intros y Hin. unfold Ensembles.In, Range in *. inv Hin.
                   eapply Hfz. eassumption. }
                  
-                eapply (conj Hbv (conj H16 (conj H15 (conj H13 (conj H12 (conj H10 (conj H11 (conj H14 Hfr')))))))). }
+                eapply (conj Hbv (conj H15 (conj H14 (conj H12 (conj H11 (conj H9 (conj H10 (conj H13 Hfr')))))))). }
 
               eapply pre_curry_l. intros Hbv. 
               eapply pre_curry_l. intros Hrel. eapply pre_curry_l. intros Hcase. eapply pre_curry_l. intros Hfv. eapply pre_curry_l. intros Hun.
               
-              assert (Hdisr : Disjoint var (S \\ [set z] \\ bound_var ei :|: (bound_var e :|: bound_var_fun_map' fm)) [set r]).
+              assert (Hdisr : Disjoint var (S \\ [set z] \\ bound_var ei :|: (bound_var e :|: bound_var_fun_map fm)) [set r]).
               { edestruct inline_letapp_var_eq. eassumption.
                 - subst. eapply Union_Disjoint_l. now sets. eapply Disjoint_sym.
                   eapply Disjoint_Included_l. eapply Singleton_Included. eapply HSin.
                   repeat normalize_bound_var_in_ctx. repeat normalize_occurs_free_in_ctx.
                   eapply Disjoint_Included_r; [ | eapply Hdis2 ]. now sets. 
                 - repeat normalize_bound_var_in_ctx. repeat normalize_occurs_free_in_ctx.
-                  inv H10.
+                  inv H9.
                   + eapply Disjoint_Included_r. eapply Singleton_Included. eassumption. eapply Union_Disjoint_l.
                     * sets.
                     * eapply Disjoint_Included_r. eassumption. eapply Disjoint_sym.
@@ -1747,8 +1436,7 @@ Section Inline_correct.
                     eapply image_apply_r_set. eapply Union_Disjoint_r. now sets.
                     eapply Disjoint_Included; [| | eapply Hdis2 ]. rewrite Setminus_Union_distr. now sets. now sets.
                   + repeat normalize_bound_var_in_ctx. repeat normalize_occurs_free_in_ctx.
-                    eapply Disjoint_Included_l; [| eapply Hdis3 ]. simpl. rewrite Setminus_Union_distr. xsets.
-                  + sets.
+                    eapply Disjoint_Included_l; [| eapply Hdis3 ]. simpl. sets.
                   + eapply Disjoint_Included_r. eapply bound_var_occurs_free_Eletapp_Included. eassumption.
                   + (* Make lemma if needed about fun_map_vars fm S (set_list (combine xs (apply_r_list sig l)) sig) *)
                     intros ? ? ? ? ?. edestruct Hfm; eauto. destructAll.
@@ -1761,7 +1449,7 @@ Section Inline_correct.
                 * zify; omega.
                 * eapply (proj1 (ub_app_ctx_f e')). split; [| split ]; [| eassumption |].
                   eapply unique_bindings_inline_letapp; [ eassumption | | eassumption ].
-                  intros Hc. eapply H12 in Hc.
+                  intros Hc. eapply H11 in Hc.
                   unfold Ensembles.In, Range in Hc, Hfr. zify; omega.
                   eapply Disjoint_Included_l. eapply bound_var_inline_letapp. eassumption.
                   eapply Union_Disjoint_l.
@@ -1772,8 +1460,8 @@ Section Inline_correct.
                 * eapply Included_trans. eapply occurs_fee_inline_letapp. eassumption.
                   assert (Hsub : occurs_free ei :|: (occurs_free e' \\ stemctx.bound_stem_ctx C) \subset
                                              occurs_free ei :|: (occurs_free e' \\ [set r])).
-                  { edestruct inline_letapp_var_eq_alt. eassumption. inv H20; subst. now sets.
-                    inv H20. now sets. rewrite Union_Setminus_Included with (s3 := [set r]); tci. sets.
+                  { edestruct inline_letapp_var_eq_alt. eassumption. inv H19; subst. now sets.
+                    inv H19. now sets. rewrite Union_Setminus_Included with (s3 := [set r]); tci. sets.
                     sets. }
                   eapply Included_trans. eassumption. eapply Union_Included.
                   -- eapply Included_trans. eassumption. eapply Included_trans.
@@ -1802,9 +1490,9 @@ Section Inline_correct.
                   -- eassumption.
                   -- eassumption.
                   -- eauto.
-                  -- simpl. intros. edestruct H21 with (f0 := f). constructor. now left. eassumption. eassumption.
+                  -- simpl. intros. edestruct H20 with (f0 := f). constructor. now left. eassumption. eassumption.
                      destructAll. do 2 subst_exp. eapply Hrel.
-                     ++ edestruct preord_env_P_inj_get_list_l. now eapply H20. normalize_occurs_free. now sets.
+                     ++ edestruct preord_env_P_inj_get_list_l. now eapply H19. normalize_occurs_free. now sets.
                         eassumption. destructAll.                           
                         eapply preord_env_P_inj_set_lists_l'; try eassumption.
                         eapply preord_env_P_inj_monotonic; [| eassumption ]. omega.
@@ -1816,8 +1504,8 @@ Section Inline_correct.
                         ** eassumption.
                         ** eapply Union_Disjoint_r. now sets. rewrite Dom_map_remove. sets. 
                         ** rewrite Union_Setminus_Included. sets. tci. sets. 
-                  -- intros. edestruct H21 with (f0 := f). constructor. now left. eassumption. eassumption.
-                     destructAll. subst_exp. eapply H19.
+                  -- intros. edestruct H20 with (f0 := f). constructor. now left. eassumption. eassumption.
+                     destructAll. subst_exp. eapply H18.
                      ++ rewrite apply_r_set_f_eq. eassumption.
                      ++ eapply fun_map_inv_antimon.
                         2:{ eapply Included_trans. eapply Included_Union_Setminus with (s2 := [set x]); tci.
@@ -1832,13 +1520,11 @@ Section Inline_correct.
                            normalize_bound_var_ctx. normalize_sets. intros y Hin Hin'.
                            eapply bound_var_inline_letapp in Hin'; [| eassumption ]. eapply Hdis2.
                            constructor. 2:{ right. rewrite image_Union. right. eassumption. }
-                           inv Hin'. inv H30.
+                           inv Hin'. inv H29.
                            eapply Hfx. unfold Ensembles.In, Range in *. zify; omega.
-                           eapply H12 in H30. eapply Hfx. unfold Ensembles.In, Range in *. zify; omega.
+                           eapply H11 in H29. eapply Hfx. unfold Ensembles.In, Range in *. zify; omega.
                         ** eassumption.
-                        ** intros Hc. eapply Hdis3. constructor. 2:{ now left; eauto. }
-                           normalize_bound_var. simpl. rewrite Setminus_Union_distr. right.
-                           constructor. reflexivity. intros Hc1. eapply H1. eapply funname_in_exp_subset. eassumption.
+                        ** intros Hc. eapply Hdis3. constructor. 2:{ eassumption. } now eauto.
                         ** intros Hc. eapply Hdis1. constructor. now constructor. now eauto.
                         ** intros Hc. inv Hc; eauto.
                   -- eassumption.
@@ -1846,13 +1532,13 @@ Section Inline_correct.
                      eapply Disjoint_Included_l. eapply bound_var_inline_letapp. eassumption.
                      eapply Disjoint_Included; [| | eapply Hdis2 ]. normalize_occurs_free. rewrite image_Union. now sets.
                      eapply Union_Included. intros u Hc. inv Hc. eapply Hfx. unfold Ensembles.In, Range in *. zify; omega.
-                     intros u Hc. eapply H12 in Hc. unfold Ensembles.In, Range in *. eapply Hfx. zify; omega.
+                     intros u Hc. eapply H11 in Hc. unfold Ensembles.In, Range in *. eapply Hfx. zify; omega.
                   -- intros Hc. eapply Hdis1'. normalize_occurs_free. normalize_bound_var.
                      constructor. now eauto. rewrite !image_Union. now eauto.
              + eapply post_weakening. 
                 2:{ eapply pre_transfer_r. eapply pre_strenghtening. 2:{
                       eapply post_weakening; [| eassumption ]. simpl. intros.
-                      eapply (conj H10 H11). }
+                      eapply (conj H9 H10). }
                     simpl. intros.  destructAll. eapply fresh_monotonic; [| eassumption ]. sets. }
                 simpl. intros. destructAll.
                 split; [| split; [| split; [| split; [| split ]]]]; eauto.
@@ -1866,16 +1552,16 @@ Section Inline_correct.
       eapply bind_triple. eapply pre_transfer_r. now eapply get_names_lst_fresh. intros xs w. simpl.
       eapply pre_curry_l. intros Hf. eapply pre_curry_l. intros Hnd.  eapply pre_curry_l. intros Hlen.
 
-      assert (Hsame1 : bound_var_fundefs f2 \\ funname_in_fundefs f2 \\ name_in_fundefs f2 \subset bound_var (Efun f2 e) \\ funname_in_exp (Efun f2 e)).
-      { normalize_bound_var. simpl. rewrite !Setminus_Union_distr. eapply Included_Union_preserv_l.
-        rewrite <- !Setminus_Union. eapply Included_Setminus; [| now sets ].
-        eapply Disjoint_Included_r. eapply funname_in_exp_subset. sets. } 
+      (* assert (Hsame1 : bound_var_fundefs f2 \\ funname_in_fundefs f2 \\ name_in_fundefs f2 \subset bound_var (Efun f2 e) \\ funname_in_exp (Efun f2 e)). *)
+      (* { normalize_bound_var. simpl. rewrite !Setminus_Union_distr. eapply Included_Union_preserv_l. *)
+      (*   rewrite <- !Setminus_Union. eapply Included_Setminus; [| now sets ]. *)
+      (*   eapply Disjoint_Included_r. eapply funname_in_exp_subset. sets. }  *)
 
-      assert (Hsame2 : bound_var e \\ funname_in_exp e \subset bound_var (Efun f2 e) \\ funname_in_exp (Efun f2 e)).
-      { normalize_bound_var. simpl. rewrite !Setminus_Union_distr. eapply Included_Union_preserv_r.
-        rewrite (Union_commut _ (funname_in_exp _)). rewrite <- Setminus_Union. eapply Included_Setminus; [| now sets ].
-        eapply Disjoint_Included_r. eapply Union_Included. eapply funname_in_fundefs_subset.
-        eapply name_in_fundefs_bound_var_fundefs. sets. } 
+      (* assert (Hsame2 : bound_var e \\ funname_in_exp e \subset bound_var (Efun f2 e) \\ funname_in_exp (Efun f2 e)). *)
+      (* { normalize_bound_var. simpl. rewrite !Setminus_Union_distr. eapply Included_Union_preserv_r. *)
+      (*   rewrite (Union_commut _ (funname_in_exp _)). rewrite <- Setminus_Union. eapply Included_Setminus; [| now sets ]. *)
+      (*   eapply Disjoint_Included_r. eapply Union_Included. eapply funname_in_fundefs_subset. *)
+      (*   eapply name_in_fundefs_bound_var_fundefs. sets. }  *)
 
       
       assert (Hfm' : fun_map_vars (add_fundefs f2 fm) (S \\ FromList xs) (set_list (combine (all_fun_name f2) xs) sig)).
@@ -1884,9 +1570,7 @@ Section Inline_correct.
           eapply Disjoint_Included; [| | eapply Hdis1 ]; sets.
         + repeat normalize_bound_var_in_ctx. repeat normalize_occurs_free_in_ctx. sets.
         + repeat normalize_bound_var_in_ctx. repeat normalize_occurs_free_in_ctx. sets.
-        + repeat normalize_bound_var_in_ctx. repeat normalize_occurs_free_in_ctx. xsets.
-        + sets.
-        + sets. }
+        + repeat normalize_bound_var_in_ctx. repeat normalize_occurs_free_in_ctx. xsets. }
 
       assert (Hnd' := NoDup_all_fun_name _ H2).
       assert (Hseq :  apply_r_list (set_list (combine (all_fun_name f2) xs) sig) (all_fun_name f2) = xs).
@@ -1897,8 +1581,6 @@ Section Inline_correct.
         - eassumption.
         - repeat normalize_occurs_free_in_ctx. repeat normalize_bound_var_in_ctx. eapply Union_Disjoint_r.
           eapply Disjoint_Included; [| | eapply Hdis1 ]; now sets.
-          (* eapply Disjoint_Included_r. eapply Included_Setminus_compat. eapply occurs_free_fun_map_add_fundefs. reflexivity. *)
-          (* rewrite !Setminus_Union_distr. rewrite Setminus_Same_set_Empty_set. normalize_sets.  *)
           eapply Disjoint_Included; [| | eapply Hdis1 ]; now sets.
         - eapply Disjoint_Included_r.
           + eapply Included_trans. eapply image_apply_r_set_list. now eauto.
@@ -1910,22 +1592,12 @@ Section Inline_correct.
               normalize_bound_var. now sets.
         - repeat normalize_occurs_free_in_ctx. repeat normalize_bound_var_in_ctx. eapply Union_Disjoint_r.
           + sets.
-            (* eapply Union_Disjoint_r. sets. eapply Disjoint_Included_r. eapply bound_var_fun_map_add_fundefs_un'. eassumption. xsets. *)
           + eapply Disjoint_Included_r. eapply image_apply_r_set_list. now eauto.
             rewrite <- Same_set_all_fun_name. rewrite !Setminus_Union_distr. rewrite !image_Union. 
             repeat (eapply Union_Disjoint_r; sets).
             now xsets.
             now xsets.
-            (* eapply Disjoint_Included_r. eapply image_monotonic. eapply Included_Setminus_compat. eapply occurs_free_fun_map_add_fundefs. reflexivity. *)
-            (* rewrite !Setminus_Union_distr.  rewrite !Setminus_Same_set_Empty_set. repeat normalize_sets. now xsets. *)
-        - repeat normalize_occurs_free_in_ctx. repeat normalize_bound_var_in_ctx.
-          eapply Union_Disjoint_r.
-          + eapply Disjoint_Included; [| | eapply Hdis3 ]. now sets.
-            rewrite Setminus_Union. rewrite Union_commut. rewrite <- Setminus_Union. eassumption.
-          + eapply Disjoint_Included_r. now sets.
-            eapply Disjoint_Included; [| | eapply Hdis3 ]. now sets.
-            rewrite Setminus_Union. rewrite Union_commut. rewrite <- Setminus_Union. eassumption.
-        - sets.
+        - repeat normalize_occurs_free_in_ctx. repeat normalize_bound_var_in_ctx. sets.
         - repeat normalize_occurs_free_in_ctx. repeat normalize_bound_var_in_ctx. sets.
         - eapply fun_map_vars_set_list. eassumption.
         - rewrite Hseq. eassumption.
@@ -1947,7 +1619,7 @@ Section Inline_correct.
                 rewrite !Setminus_Union_distr. rewrite !Setminus_Same_set_Empty_set. repeat normalize_sets. now sets.
                 eapply Disjoint_Included_r. eapply name_in_fundefs_bound_var_fundefs. now sets.
             + repeat normalize_bound_var_in_ctx. repeat normalize_occurs_free_in_ctx.
-              eapply Disjoint_Included_l. eapply Included_Union_compat. reflexivity. eapply bound_var_fun_map_add_fundefs_un'. eassumption. 
+              eapply Disjoint_Included_l. eapply Included_Union_compat. reflexivity. eapply bound_var_fun_map_add_fundefs_un. eassumption. 
               eapply Disjoint_Included_r. 
               eapply image_apply_r_set_list. now eauto. eapply Union_Disjoint_r.
               * eapply Disjoint_sym. eapply Disjoint_Included; [| | eapply Hdis2 ]. now sets. eassumption.
@@ -1960,7 +1632,7 @@ Section Inline_correct.
                 eapply Disjoint_Included; [| | eapply Hdis1' ]. now sets. now sets.
             + repeat normalize_bound_var_in_ctx. repeat normalize_occurs_free_in_ctx. eapply Union_Disjoint_r. eapply Union_Disjoint_r. 
               now sets.
-              eapply Disjoint_Included_r. eapply bound_var_fun_map_add_fundefs_un'. eassumption. now xsets.
+              eapply Disjoint_Included_r. eapply bound_var_fun_map_add_fundefs_un. eassumption. now xsets.
               eapply Disjoint_Included_r. 
               eapply image_apply_r_set_list. now eauto. eapply Union_Disjoint_r.
               * now sets.
@@ -1973,18 +1645,11 @@ Section Inline_correct.
                 eapply Disjoint_Included; [| | eapply Hdis2 ]. now sets. now sets.
             + repeat normalize_bound_var_in_ctx. repeat normalize_occurs_free_in_ctx.
               rewrite Dom_map_add_fundefs. eapply Union_Disjoint_r.
-              * eapply Union_Disjoint_r.
-                -- eapply Disjoint_Included_r. eapply name_in_fundefs_bound_var_fundefs. now sets.
-                -- eapply Disjoint_Included; [| | eapply Hdis3 ]; sets.
-              * eapply Disjoint_Included_r. eapply funname_fun_map_add_fundefs. eapply Union_Disjoint_r.
-                -- eapply Disjoint_Included_r. eapply funname_in_fundefs_subset. sets.
-                -- eapply Disjoint_Included; [| | eapply Hdis3 ]. now sets. eassumption.
-            + eapply Disjoint_Included_r. eapply bound_var_fun_map_add_fundefs_un. eassumption. eapply Union_Disjoint_r.
-              * eapply Disjoint_Included_l. eapply funname_in_exp_subset. sets.
+              * eapply Disjoint_Included_r. eapply name_in_fundefs_bound_var_fundefs. now sets.
               * sets.
             + repeat normalize_bound_var_in_ctx. repeat normalize_occurs_free_in_ctx.
               eapply Disjoint_Included_l.
-              * eapply bound_var_fun_map_add_fundefs_un'. eassumption.
+              * eapply bound_var_fun_map_add_fundefs_un. eassumption.
               * eapply Union_Disjoint_l.
                 -- eapply Union_Disjoint_r. now sets.
                    eapply Disjoint_Included_r.
@@ -2022,10 +1687,6 @@ Section Inline_correct.
            eapply Included_Union_preserv_l. rewrite <- Same_set_all_fun_name.
            rewrite Setminus_Union_distr. rewrite !image_Union. eapply Union_Included. now sets.
            sets.
-           (* eapply Included_trans. eapply image_monotonic. eapply Included_Setminus_compat. *)
-           (* eapply occurs_free_fun_map_add_fundefs. reflexivity. *)
-           (* rewrite !Setminus_Union_distr, Setminus_Same_set_Empty_set. repeat normalize_sets. *)
-           (* rewrite image_Union. now xsets. *)
         -- eapply Included_trans. eapply Included_Setminus_compat. eassumption. reflexivity.
            eapply Setminus_Included_Included_Union. 
            eapply Included_trans. eapply image_apply_r_set_list. now eauto.
@@ -2085,18 +1746,14 @@ Section Inline_correct.
                   - eapply unique_bindings_fun_in_fundefs. eapply find_def_correct. eassumption. eassumption. }
                 eapply fun_map_inv_antimon. eapply fun_map_inv_set_lists; [ | | | now eauto ].
                 eapply fun_map_inv_set_lists_r; [| | now eauto ]. 
-                -- rewrite <- Hseq. rewrite <- H13. eapply fun_map_inv_sig_extend_Disjoint. admit. 
-                   (* eapply fun_map_inv_def_funs. *)
-                   (* eapply fun_map_inv_i_mon. eassumption. omega. eapply preord_env_P_inj_antimon. *)
-                   (* rewrite H13. rewrite Hseq. eapply IHi. eassumption. omega. normalize_occurs_free. now sets. *)
-                   (* eassumption. normalize_occurs_free. now sets. *)
-                   (* eapply Disjoint_Included; [| | eapply Hdis1 ]. now sets. normalize_bound_var. *)
-                   (* eapply Included_trans. eapply name_in_fundefs_bound_var_fundefs. now sets. *)
-                   
-                   (* rewrite Same_set_all_fun_name, H13, Hseq. eapply Disjoint_Included ; [| | eapply Hdis2 ]. now sets. eassumption. *)
-                (* eapply Disjoint_Included_r. eapply occurs_free_fun_map_add_fundefs. eassumption. *)
-                   sets.
-                   (* SearchAbout ys1. *)
+                -- rewrite <- Hseq. rewrite <- H13. eapply fun_map_inv_sig_extend_Disjoint.
+                   eapply fun_map_inv_def_funs. eapply fun_map_inv_i_mon. eassumption. omega.
+                   ++ eapply Disjoint_Included; [| | eapply Hdis1 ]. now sets. normalize_bound_var.
+                      eapply Included_trans. eapply name_in_fundefs_bound_var_fundefs. now sets.
+                   ++ rewrite Same_set_all_fun_name, H13, Hseq. eapply Disjoint_Included ; [| | eapply Hdis2 ]. now sets. eassumption.
+                   ++ eapply Disjoint_Included_l; [| eapply Hdis3 ]. normalize_bound_var.
+                      eapply Included_trans. eapply name_in_fundefs_bound_var_fundefs. now sets.
+                   ++ sets.
                 -- rewrite image_f_eq_subdomain.
                    2:{ rewrite apply_r_set_list_f_eq. eapply f_eq_subdomain_extend_lst_Disjoint. sets. }
 
@@ -2105,18 +1762,13 @@ Section Inline_correct.
                    eapply Disjoint_Included_l. eassumption. now sets.
                    rewrite <- Same_set_all_fun_name. 
                    eapply Disjoint_Included_l. eassumption.
-                   (* eapply image_monotonic. eapply Included_Setminus_compat. eapply occurs_free_fun_map_add_fundefs. reflexivity. *)
-                   (* rewrite !Setminus_Union_distr. rewrite Setminus_Same_set_Empty_set. repeat normalize_sets. *)
                    eapply Disjoint_Included; [| | eapply Hdis2 ]. normalize_occurs_free. now sets. now sets.
                 -- eapply unique_bindings_fun_in_fundefs. eapply find_def_correct. eassumption. eassumption.
                 -- eapply Union_Disjoint_r. now sets.
-                   eapply Disjoint_Included; [| | eapply Hdis3 ]. now sets.
-                   eapply Included_trans. eapply fun_in_fundefs_FromList_subset. eapply find_def_correct. eassumption. eassumption.
-                   normalize_bound_var. simpl. rewrite Setminus_Union_distr. eapply Included_Union_preserv_l.
-                   rewrite <- !Setminus_Union. eapply Included_Setminus; [| now sets ]. eapply Disjoint_Included_r.
-                   eapply funname_in_exp_subset. now sets.
-                -- sets.
-                   (* normalize_occurs_free. sets. *)
+                   eapply Disjoint_Included; [| | eapply Hdis3 ]. now sets. repeat normalize_bound_var.
+                   eapply Included_Union_preserv_l.  
+                   eapply Included_trans; [| eapply fun_in_fundefs_bound_var_fundefs; eapply find_def_correct; eauto ]. now sets.
+                -- normalize_occurs_free. sets.
           - inv HIn. contradiction. rewrite def_funs_neq in Hgetx; [| eassumption ]. eapply Henv in Hgetx; [| eassumption ]. destructAll. 
             eexists. rewrite apply_r_set_list_f_eq. rewrite extend_lst_gso. rewrite def_funs_neq. 
             split; eauto. eapply preord_val_monotonic. eassumption. omega. 
@@ -2129,7 +1781,7 @@ Section Inline_correct.
         eapply H9.
         -- eapply preord_env_P_inj_antimon. eassumption. normalize_occurs_free.
            rewrite !Union_assoc. rewrite Union_Setminus_Included; sets. tci.
-        -- eapply fun_map_inv_antimon. rewrite <- Hseq. rewrite <- H13. eapply fun_map_inv_def_funs.
+        -- eapply fun_map_inv_antimon. rewrite <- Hseq. rewrite <- H13. eapply fun_map_inv_def_funs_add_fundefs.
            eapply fun_map_inv_i_mon. eassumption. omega. rewrite H13, Hseq. eapply preord_env_P_inj_antimon.
            eassumption. normalize_occurs_free. now sets. eassumption. normalize_occurs_free. sets.
            eapply Disjoint_Included_l. eapply name_in_fundefs_bound_var_fundefs.
@@ -2165,59 +1817,69 @@ Section Inline_correct.
                      unfold apply_r_list. rewrite list_length_map. eassumption.
                      normalize_occurs_free. rewrite !image_Union. rewrite FromList_apply_list.
                      eapply Union_Included. now sets.
-                     rewrite !Setminus_Union_distr. rewrite !image_Union. eapply Included_Union_preserv_r.
-                     eapply Union_Included; [| now sets ].
-                     eapply image_monotonic. intros z Hin. do 4 eexists; split; eauto.
+                     rewrite !Setminus_Union_distr. rewrite !image_Union.
+                     eapply Included_Union_preserv_r. eapply Union_Included.
+                     eapply image_monotonic. eapply occurs_free_fun_map_get. eassumption.
+                     eapply image_monotonic. eapply Included_trans. eapply Setminus_Included.
+                     eapply occurs_free_fun_map_remove. 
                   ** eauto.
                   ** intros. eapply preord_exp_app_l.
                      --- eauto.
                      --- eauto.
-                     --- intros. assert (Hf := H15). assert (Heqf' := Heqf). edestruct H15; eauto. destructAll.
-                         do 2 subst_exp. eapply H13.
-                         +++ edestruct preord_env_P_inj_get_list_l. now eapply H14. normalize_occurs_free. now sets.
+                     --- intros. assert (Hf := H16). assert (Heqf' := Heqf).
+                         edestruct H16; eauto. destructAll.
+                         do 2 subst_exp. eapply H14.
+                         +++ edestruct preord_env_P_inj_get_list_l. now eapply H15. normalize_occurs_free. now sets.
                              eassumption. destructAll.                           
                              eapply preord_env_P_inj_set_lists_l'; try eassumption.
                          +++ eapply fun_map_inv_antimon. eapply fun_map_inv_set_lists; [ | | | eassumption ].
-                             *** eapply fun_map_inv_sig_extend_Disjoint. rewrite <- fun_map_inv_eq in *. eassumption.
-                                 eapply Disjoint_Included_l. eapply Included_trans; [| eapply bound_var_fun_map_get'; eauto ]. now sets.
-                                 admit.
+                             *** eapply fun_map_inv_sig_extend_Disjoint. rewrite <- fun_map_inv_eq in *.
+                                 eapply fun_map_inv_remove. eassumption.
+                                 now sets.
                              *** eassumption.
-                             *** eapply Union_Disjoint_r.
-                                 eapply Disjoint_Included_l. eapply Included_trans; [| eapply bound_var_fun_map_get'; eauto ]. now sets.
-                                 admit. 
-                                 clear H25. xsets.
+                             *** eapply Union_Disjoint_r. now sets.
+                                 rewrite Dom_map_remove. sets.
                              *** rewrite Union_Setminus_Included. sets. tci. sets.
                ++ omega.
                ++ eassumption.
-               ++ eapply Union_Disjoint_r. now sets. admit.
+               ++ eapply Union_Disjoint_r. eapply Disjoint_Included; [| | eapply H1 ]; now sets.
+                  sets. 
                ++ eapply Disjoint_Included_r. eapply image_apply_r_set_list.
                   unfold apply_r_list. rewrite list_length_map. eassumption.
                   eapply Union_Disjoint_r.
                   eapply Disjoint_Included; [ | | eapply Hdis1' ]. normalize_occurs_free.
                   rewrite !image_Union. rewrite FromList_apply_list. now sets.
-                  eapply Union_Included; [| now sets ].
-                  eapply Included_Union_preserv_r. eapply Included_trans; [| eapply bound_var_fun_map_get'; eauto ]. now sets.
+                  eapply Included_Union_preserv_r. 
+                  eapply Union_Included; [| now eapply bound_var_fun_map_remove ]. 
+                  eapply Included_trans; [| eapply bound_var_fun_map_get; eauto ]. now sets.
                   rewrite Setminus_Union_distr. rewrite !image_Union. eapply Union_Disjoint_r.
-                  eapply Disjoint_Included; [| | eapply Hdis1' ]. eapply image_monotonic. eapply Included_Union_preserv_r.
+                  eapply Disjoint_Included; [| | eapply Hdis1' ].
+                  eapply image_monotonic. eapply Included_Union_preserv_r.
                   eapply occurs_free_fun_map_get. eassumption.
-                  eapply Included_Union_preserv_r. eapply Union_Included; [| now sets ].
-                  eapply Included_trans; [| eapply bound_var_fun_map_get'; eauto ]. now sets.
-                  eapply Disjoint_Included; [| | eapply Hdis1' ]. eapply image_monotonic. eapply Included_Union_preserv_r. now sets.
-                  eapply Included_Union_preserv_r. eapply Union_Included; [| now sets ].
-                  eapply Included_trans; [| eapply bound_var_fun_map_get'; eauto ]. now sets.
-               ++ eapply Union_Disjoint_r. eapply Union_Disjoint_r. now sets.
-                  clear H5. now sets.
+                  eapply Included_Union_preserv_r.
+                  eapply Union_Included; [| now eapply bound_var_fun_map_remove ].
+                  eapply Included_trans; [| eapply bound_var_fun_map_get; eauto ]. now sets.
+                  eapply Disjoint_Included; [| | eapply Hdis1' ]. eapply image_monotonic. eapply Included_Union_preserv_r.
+                  eapply Included_trans. eapply Setminus_Included. now eapply occurs_free_fun_map_remove.
+                  eapply Included_Union_preserv_r. eapply Union_Included; [| now eapply bound_var_fun_map_remove ].
+                  eapply Included_trans; [| eapply bound_var_fun_map_get; eauto ]. now sets.
+               ++ eapply Union_Disjoint_r.
+                  eapply Union_Disjoint_r. now sets.
+                  clear H6. eapply Disjoint_Included_r. eapply bound_var_fun_map_remove. now sets.
                   eapply Disjoint_Included_r. eapply image_apply_r_set_list.
                   unfold apply_r_list. rewrite list_length_map. eassumption.
-                  eapply Disjoint_Included; [ | | eapply Hdis2 ]. normalize_occurs_free.
-                  rewrite !image_Union. rewrite FromList_apply_list.
-                  eapply Union_Included; [ now sets  | ]. rewrite Setminus_Union_distr, !Union_assoc. eapply Included_Union_preserv_r.
-                  rewrite !image_Union. eapply Union_Included; [| now sets ].
-                  eapply image_monotonic.
-                  eapply occurs_free_fun_map_get. eassumption. now sets.
+                  eapply Disjoint_Included_r; [ | eapply Hdis2 ]. normalize_occurs_free.
+                  rewrite FromList_apply_list.
+                  eapply Union_Included; [ now sets  | ].
+                  rewrite Setminus_Union_distr. eapply Included_Union_preserv_r. eapply image_monotonic.
+                  eapply Included_Union_preserv_r.
+                  eapply Union_Included; [| ].
+                  eapply occurs_free_fun_map_get. eassumption.
+                  eapply Included_trans. eapply Setminus_Included. eapply occurs_free_fun_map_remove. 
+               ++ rewrite Dom_map_remove. sets.
                ++ sets.
-               ++ sets.
-               ++ (* Make lemma if needed about fun_map_vars fm S (set_list (combine xs (apply_r_list sig l)) sig) *)
+               ++ eapply fun_map_vars_inv_remove. 
+                 (* Make lemma if needed about fun_map_vars fm S (set_list (combine xs (apply_r_list sig l)) sig) *)
                   intros ? ? ? ? ?. edestruct Hfm; eauto. destructAll.
                   repeat (split; [ now eauto |]). eapply Union_Disjoint_r. now sets.
                   eapply Disjoint_Included_r. eapply image_apply_r_set_list.
@@ -2286,7 +1948,7 @@ Section Inline_correct.
         eapply Disjoint_Included; [| | eapply Hdis2 ].
         rewrite Setminus_Union_distr. rewrite !image_Union. now xsets. now sets.
       + eapply Disjoint_Included_l; [| eassumption ]. normalize_bound_var. sets.
-      + eassumption.
+      + eapply Disjoint_Included_r. eapply bound_var_occurs_free_Eprim_Included. eassumption.
       + eapply fun_map_vars_set. eassumption.
       + intros e' w2. eapply return_triple.
         intros _ st'. intros [Hf1 [Hf2 [Hf3 [Hf4 [Hun [Hsub [Hsub' Hsem]]]]]]].
@@ -2355,14 +2017,8 @@ Section Inline_correct.
           now sets. now sets. now sets. eapply Disjoint_Included; [| | eapply Hnames2 ]. rewrite FromList_apply_list. rewrite Same_set_all_fun_name.
           reflexivity. now sets.
         - eapply Disjoint_Included_l; [| eassumption ].
-          normalize_bound_var. simpl. rewrite !Setminus_Union_distr. do 2 eapply Included_Union_preserv_r.
-          eapply Included_Union_preserv_l. rewrite !Setminus_Union. rewrite Union_commut.
-          rewrite <- Union_assoc. rewrite <- Setminus_Union. eapply Included_Setminus; [| now sets ].
-          eapply Union_Disjoint_r; [| eapply Union_Disjoint_r ]; sets.
-          + eapply Disjoint_Included_r. eapply funname_in_fundefs_subset. sets.
-          + eapply Disjoint_Included_r. eapply name_in_fundefs_bound_var_fundefs. sets.
-        - repeat normalize_occurs_free_in_ctx. repeat normalize_bound_var_in_ctx. 
-          sets.
+          normalize_bound_var. now sets.
+        - eapply Disjoint_Included_r. eapply bound_var_occurs_free_Fcons_Included. eassumption.
         - repeat normalize_occurs_free_in_ctx. repeat normalize_bound_var_in_ctx.
           eapply fun_map_vars_set_list. eassumption. }
 
@@ -2390,15 +2046,11 @@ Section Inline_correct.
               eapply Disjoint_Included; [| | eapply Hdis2 ]. eapply Included_Union_preserv_r.
               eapply image_monotonic. rewrite !Setminus_Union_distr. now sets. now sets.
               eapply Disjoint_Included; [| | eapply Hnames2 ]. rewrite FromList_apply_list, <- Same_set_all_fun_name. simpl. now sets. now sets.
-            + repeat normalize_bound_var_in_ctx. repeat normalize_occurs_free_in_ctx.
-              eapply Disjoint_Included_l; [| eapply Hdis3 ]. simpl. rewrite !Setminus_Union_distr.
-              do 3 eapply Included_Union_preserv_r. rewrite !Setminus_Union.
-              rewrite (Union_commut (funname_in_exp e)). rewrite <- !Union_assoc. rewrite (Union_commut [set v]). 
-              rewrite Union_assoc. rewrite <- Union_assoc. rewrite <- Setminus_Union. rewrite <- Setminus_Union.
-              eapply Included_Setminus; [| now sets ]. eapply Union_Disjoint_r.
-              * eapply Disjoint_Included_r. eapply funname_in_exp_subset. sets.
-              * sets.
-            + sets.
+            + repeat normalize_bound_var_in_ctx. repeat normalize_occurs_free_in_ctx. sets.
+            + eapply Disjoint_Included_r; [| eassumption ].
+              normalize_bound_var. normalize_occurs_free.
+              eapply Union_Included. now sets. rewrite !Union_assoc. rewrite Union_commut.
+              rewrite <- Union_Included_Union_Setminus. sets. tci. sets.              
             + eapply fun_map_vars_antimon; eauto. sets.
             + simpl in Hnames1. inv Hnames1. eassumption.
             + eapply Disjoint_Included; [ | | eapply Hnames2 ]; simpl; sets. normalize_sets. sets. normalize_bound_var. now sets. } 
@@ -2509,13 +2161,6 @@ Section Inline_correct.
     intros x Hin. inv Hin. destructAll. rewrite M.gempty in H. inv H.
   Qed.
 
-  Lemma fun_name__fun_map_empty :
-    funname_fun_map (M.empty _) <--> Empty_set _.
-  Proof.
-    split; sets.
-    intros x Hin. inv Hin. destructAll. rewrite M.gempty in H. inv H.
-  Qed.
-
   Lemma bound_var_fun_map_empty :
     bound_var_fun_map (M.empty _) <--> Empty_set _.
   Proof.
@@ -2535,39 +2180,47 @@ Section Inline_correct.
       occurs_free e' \subset occurs_free e /\
       (forall k,
           preord_env_P cenv PG (occurs_free e) k rho1 rho2 ->
-          Disjoint _ (bound_var e) (Dom_map rho1) ->
           preord_exp cenv P1 PG k (e, rho1) (e', rho2)).
   Proof.
     intros. edestruct (inline_correct_mut d) as [He _].
     unfold beta_contract_top, triple in *.
+    
     specialize (He e (M.empty _) (M.empty _) st
-                   (fun x => Pos.max (max_var e 1%positive) (List_util.max_list (map fst (M.elements rho1)) 1%positive) < x) H H0).
+                   (fun x => Pos.max (max_var e 1%positive) (List_util.max_list (map fst (M.elements rho1)) 1%positive) < x) H).
 
+    rewrite occurs_free_fun_map_empty, bound_var_fun_map_empty in *.
+    repeat normalize_sets.
+    specialize (He H0).
+
+
+    assert (Hdis : Disjoint var (bound_var e) (image (apply_r (M.empty var)) (occurs_free e))).
+    { rewrite image_apply_r_empty. sets. } 
+
+    
     assert (Hdis1 : Disjoint var (fun x : var => Pos.max (max_var e 1) (List_util.max_list (map fst (M.elements rho1)) 1) < x)
-                             (bound_var e :|: image (apply_r (M.empty var))
-                                        (occurs_free e :|: occurs_free_fun_map
-                                                     (M.empty (fun_tag * list var * exp))))).
-    { rewrite apply_r_empty_f_eq. rewrite image_id. rewrite occurs_free_fun_map_empty. normalize_sets. 
+                             (bound_var e :|: image (apply_r (M.empty var)) (occurs_free e))).
+    { rewrite apply_r_empty_f_eq. rewrite image_id.  
       constructor. intros x Hnin. inv Hnin. inv H4. 
       eapply bound_var_leq_max_var with (y := 1%positive) in H5. unfold Ensembles.In in *. zify. omega.
       eapply occurs_free_leq_max_var with (y := 1%positive) in H5. unfold Ensembles.In in *. zify. omega. }
-    
-    assert (Hdis2 : Disjoint var (bound_var e \\ funname_in_exp e)
-                             (Dom_map (M.empty (fun_tag * list var * exp)) :|: funname_fun_map (M.empty (fun_tag * list var * exp)))).
-    { rewrite Dom_map_empty, fun_name__fun_map_empty. sets. }
 
-    assert (Hdis3 : Disjoint var (funname_in_exp e) (bound_var_fun_map (M.empty (fun_tag * list var * exp)))).
-    { rewrite bound_var_fun_map_empty. sets. }
+
+    
+    assert (Hdis2 : Disjoint var (bound_var e) (Dom_map (M.empty (fun_tag * list var * exp)))).
+    { rewrite Dom_map_empty. sets. }
+    
+    assert (Hdis3 :  Disjoint var (Empty_set var) (bound_var e :|: occurs_free e) ).
+    { sets. }      
 
     assert (Hfinv : fun_map_vars (M.empty (fun_tag * list var * exp))
                                  (fun x : var => Pos.max (max_var e 1) (List_util.max_list (map fst (M.elements rho1)) 1) < x)
                                  (M.empty var)).
     { unfold fun_map_vars. intros. rewrite M.gempty in H3. inv H3. }
-
+    
     assert (Hf : fresh (fun x : var => Pos.max (max_var e 1) (List_util.max_list (map fst (M.elements rho1)) 1) < x) (next_var (fst (c, tt)))).
     { unfold fresh. intros. unfold Ensembles.In in *. simpl in *. zify; omega. }
 
-    specialize (He Hdis1 Hdis2 Hdis3 Hfinv tt (c, tt) Hf).
+    specialize (He Hdis Hdis1 Hdis2 Hdis3 Hfinv tt (c, tt) Hf).
     
     unfold runState, run_compM. simpl in *. 
     
@@ -2575,22 +2228,16 @@ Section Inline_correct.
                 (beta_contract St IH d e (cps.M.empty var) (cps.M.empty (fun_tag * list var * exp)) st) tt (c, tt)) eqn:Heq.   
     
     destruct e0. contradiction. destructAll.
-
+    
     destruct p. do 2 eexists. split; [| split; [| split ]].
     - reflexivity.
     - eassumption.
     - eapply Included_trans. eassumption. rewrite apply_r_empty_f_eq. rewrite image_id, occurs_free_fun_map_empty.
       sets.
     - intros. eapply H9; eauto. rewrite apply_r_empty_f_eq.
-      intros x Hin. unfold id. eauto.
+      intros x Hin. unfold id. now eauto.
 
-      rewrite apply_r_empty_f_eq. rewrite image_id.
-      constructor. intros x Hin. inv Hin. unfold Ensembles.In in *. destruct H13.
-      eapply cps.M.elements_correct in H13.
-      eapply in_map with (f := fst) in H13. eapply List_util.max_list_spec2 with (z := 1%positive) in H13.
-      simpl in *.  zify; omega.
-
-      intro; intros. rewrite M.gempty in H13; inv H13.
+      intro; intros. rewrite M.gempty in H12; inv H12.
   Qed. 
 
 End Inline_correct.
